VLSM/Equivocators/Composition/LimitedEquivocation/FixedEquivocation.v
@@ -34,6 +34,8 @@ Context
 
 Existing Instance i0.
 
+(** Definition of fixed-equivocation for states of the composition of equivocators.
+*)
 Definition state_has_fixed_equivocation
   (s : composite_state equivocator_IM)
   : Prop
@@ -49,6 +51,9 @@ Definition equivocators_fixed_equivocations_constraint
   /\ state_has_fixed_equivocation (fst som').
 
 
+(**
+If a future state has fixed equivocation, then so must the current state.
+*)
 Lemma in_futures_reflects_fixed_equivocation
   (s1 s2 : composite_state equivocator_IM)
   (Hfutures : in_futures (pre_loaded_with_all_messages_vlsm (free_composite_vlsm equivocator_IM)) s1 s2)
@@ -70,16 +75,21 @@ Proof.
   clear -H4 H.
   destruct H4 as [_ Ht]. simpl in Ht.
   apply incl_tran with (equivocating_indices IM index_listing s); [|assumption].
-  apply equivocators_transition_reflects_equivocating_indices with iom oom l.
+  apply equivocators_transition_preserves_equivocating_indices with iom oom l.
   assumption.
 Qed.
 
-
+(** Composition of equivocators with no message equivocation and a
+fixed set of machines allowed to state-equivocate.
+*)
 Definition equivocators_fixed_equivocations_vlsm
   : VLSM message
   :=
   composite_vlsm equivocator_IM equivocators_fixed_equivocations_constraint.
 
+(**
+Inclusion in the free composition
+*)
 Lemma equivocators_fixed_equivocations_vlsm_incl_free
   : VLSM_incl equivocators_fixed_equivocations_vlsm (free_composite_vlsm equivocator_IM).
 Proof.
@@ -87,6 +97,10 @@ Proof.
   intros l som H. exact I.
 Qed.
 
+(**
+Inclusion in the composition of equivocators with no message equivocation
+(no restriction on state equivocation).
+*)
 Lemma equivocators_fixed_equivocations_vlsm_incl_no_equivocations
   : VLSM_incl equivocators_fixed_equivocations_vlsm (equivocators_no_equivocations_vlsm IM Hbs finite_index).
 Proof.
@@ -97,6 +111,10 @@ Qed.
 End equivocators_fixed_equivocations_vlsm.
 
 Section fixed_equivocation_without_fullnode.
+
+(**
+In this section we define fixed equivocation for the regular composition.
+*)
 
 Context
   {message : Type}
@@ -130,7 +148,15 @@ Context
 
 Existing Instance X_has_been_observed_capability.
 
-Definition seeded_free_equivocators_composition
+(**
+[free_equivocating_vlsm_composition] is the free composition of the subset of
+nodes which are allowed to equivocate.
+
+[pre_loaded_free_equivocating_vlsm_composition] adds to that composition as initial
+messages all initial messages of the full composition, along with those given by
+the predicate argument @messageSet@.
+*)
+Definition pre_loaded_free_equivocating_vlsm_composition
   (messageSet : message -> Prop)
   := pre_loaded_vlsm free_equivocating_vlsm_composition
       (fun m => messageSet m \/ vinitial_message_prop X m).
@@ -139,6 +165,14 @@ Context
   {validator : Type}
   .
 
+(**
+The fixed equivocation constraint for the regular composition of nodes
+stipulates that a message can be received either if receiving it satisfies 
+the [no_additional_equivocations_constraint] (message [has_been_observed],
+or it has the [initial_message_prop]erty), or it can be emited by the
+free composition of equivocators pre=loaded with with messages producing
+[no_additional_equivocations] for the current state.
+*)
 Definition fixed_equivocation_constraint
   (l : composite_label IM)
   (som : composite_state IM * option message)
@@ -147,16 +181,33 @@ Definition fixed_equivocation_constraint
   no_additional_equivocations_constraint X l som \/
   let (s, om) := som in
   exists m : message, om = Some m /\
-  can_emit (seeded_free_equivocators_composition (no_additional_equivocations X s)) m.
+  can_emit (pre_loaded_free_equivocating_vlsm_composition (no_additional_equivocations X s)) m.
 
 Existing Instance i0.
 
+(** Composition of regular VLSMs under the [fixed_equivocation_constraint].
+*)
 Definition fixed_equivocation_vlsm_composition : VLSM message
   := composite_vlsm IM fixed_equivocation_constraint.
 
 End fixed_equivocation_without_fullnode.
 
 Section fixed_equivocation_with_fullnode.
+
+(**
+This section instantiates the [full_node_condition_for_admissible_equivocators]
+by choosing the admissible indices to be the fixed set of nodes allowed to 
+equivocate, and then shows that this constraint is stronger than the
+[fixed_equivocation_constraint].
+*)
+
+
+(**
+Context setting the stage for, and instantiating the
+[full_node_condition_for_admissible_equivocators].
+It requires that the nodes have [has_been_sent] and [has_been_received]
+capabilities, that the number of nodes is finite
+*)
   Context
     {message : Type}
     (index : Type)
@@ -170,14 +221,18 @@ Section fixed_equivocation_with_fullnode.
     (finite_index : Listing index_listing)
     (equivocating : set index)
     (admissible_index := fun s i => In i equivocating)
-    (Hno_resend : forall i : index, cannot_resend_message_stepwise_prop (IM i))
     (full_node_constraint
       := full_node_condition_for_admissible_equivocators IM Hbs Hbr finite_index admissible_index)
     (full_node_constraint_alt
       := full_node_condition_for_admissible_equivocators_alt IM Hbs Hbr finite_index admissible_index)
     .
 
-  Section fixed_equivocation_constraint_comparison.
+  
+(**
+Context for the [fixed_equivocation_constraint]. Additionally to the above it
+requires that equality on messages is decidable and that the set of VLSMs
+allowed to equivocate is non-empty.
+*)
 
   Context
     `{EqDecision message}
@@ -186,12 +241,8 @@ Section fixed_equivocation_with_fullnode.
     (equivocating_IM := sub_IM IM equivocating)
     (equivocating_index_eq_dec : EqDecision equivocating_index := sub_index_eq_dec equivocating)
     (equivocating_inhabited : Inhabited equivocating_index := sub_index_i0 _ Hi0_equiv)
-    {validator : Type}
-    (A : validator -> index)
-    (sender : message -> option validator)
     (fixed_equivocation_constraint : composite_label IM  -> composite_state IM * option message -> Prop
       := fixed_equivocation_constraint IM Hbs Hbr equivocating Hi0_equiv finite_index)
-    (Hsender_safety : Prop := sender_safety_prop IM (free_constraint IM) A sender)
     (X := free_composite_vlsm IM)
     (X_has_been_sent_capability : has_been_sent_capability X := composite_has_been_sent_capability IM (free_constraint IM) finite_index Hbs)
     (X_has_been_received_capability : has_been_received_capability X := composite_has_been_received_capability IM (free_constraint IM) finite_index Hbr)
@@ -200,10 +251,36 @@ Section fixed_equivocation_with_fullnode.
 
   Existing Instance  equivocating_inhabited.
   Existing Instance  equivocating_index_eq_dec.
-
   Existing Instance X_has_been_observed_capability.
-  Lemma fixed_equivocation_constraint_subsumption :
-    preloaded_constraint_subsumption IM full_node_constraint fixed_equivocation_constraint.
+
+  (**
+  The [full_node_constraint_alt] is stronger than the [fixed_equivocation_constraint].
+  *)
+  Lemma fixed_equivocation_constraint_subsumption_alt
+    : preloaded_constraint_subsumption IM full_node_constraint_alt fixed_equivocation_constraint.
+  Proof.
+    intros s Hs l om [Hno_equiv | Hfull]; [left; assumption|].
+    destruct Hfull as [m [Hom [i [Hi Hm]]]].
+    subst om.
+    right. exists m. split; [reflexivity|].
+    remember (no_additional_equivocations (free_composite_vlsm IM) s) as P.
+    unfold pre_loaded_free_equivocating_vlsm_composition.
+    remember (fun m => P m \/ vinitial_message_prop (free_composite_vlsm IM) m) as Q.
+    specialize (can_emit_composite_free_lift equivocating_IM P Q) as Hemit.
+    spec Hemit. { intros. subst Q. left. assumption. }
+    specialize (Hemit (dec_exist _  i Hi)).
+    apply Hemit.
+    assumption.
+  Qed.
+
+  (** If all nodes have the [cannot_resend_message_stepwise_prop]erty, then the
+  full node constraint is stronger than the [fixed_equivocation_constraint].
+
+  (by reduction to the result above)
+  *)
+  Lemma fixed_equivocation_constraint_subsumption
+    (Hno_resend : forall i : index, cannot_resend_message_stepwise_prop (IM i))
+    : preloaded_constraint_subsumption IM full_node_constraint fixed_equivocation_constraint.
   Proof.
     cut (preloaded_constraint_subsumption IM full_node_constraint_alt fixed_equivocation_constraint).
     {
@@ -217,21 +294,9 @@ Section fixed_equivocation_with_fullnode.
         ); [assumption|].
       assumption.
     }
-    intros s Hs l om [Hno_equiv | Hfull]; [left; assumption|].
-    destruct Hfull as [m [Hom [i [Hi Hm]]]].
-    subst om.
-    right. exists m. split; [reflexivity|].
-    remember (no_additional_equivocations (free_composite_vlsm IM) s) as P.
-    unfold seeded_free_equivocators_composition.
-    remember (fun m => P m \/ vinitial_message_prop (free_composite_vlsm IM) m) as Q.
-    specialize (can_emit_composite_free_lift equivocating_IM P Q) as Hemit.
-    spec Hemit. { intros. subst Q. left. assumption. }
-    specialize (Hemit (dec_exist _  i Hi)).
-    apply Hemit.
-    assumption.
+    apply fixed_equivocation_constraint_subsumption_alt.
   Qed.
 
-  End fixed_equivocation_constraint_comparison.
 End fixed_equivocation_with_fullnode.
 
 Section from_equivocators_to_nodes.
@@ -278,7 +343,7 @@ Context
   (sub_equivocator_IM := sub_IM (equivocator_IM IM) equivocating)
   .
 
-Lemma not_equivocating_equivocatos_choice_fixed_descriptor_is_0
+Lemma not_equivocating_index_has_singleton_state
   (s : composite_state (equivocator_IM IM))
   (Hs : protocol_state_prop XE s)
   (i : index)
@@ -308,43 +373,55 @@ Qed.
 
 Existing Instance i0.
 
+(**
+[proper_equivocator_descriptors] strengthen for fixed-equivocation.
+We require that if the index is not equivocating, than the corresponding
+descriptor is a [zero_descriptor].
+*)
 Definition proper_fixed_equivocator_descriptors
-  (eqv_choice : equivocator_descriptors IM)
+  (eqv_descriptors : equivocator_descriptors IM)
   (s : state)
   : Prop
-  := proper_equivocator_descriptors IM eqv_choice s /\
-    forall i, ~In i equivocating -> eqv_choice i = Existing _ 0 false.
+  := proper_equivocator_descriptors IM eqv_descriptors s /\
+    forall i, ~In i equivocating -> eqv_descriptors i = Existing _ 0 false.
 
-
-Lemma not_equivocating_equivocatos_choice_proper_fixed
+(**
+[not_equivocating_equivocator_descriptors] satisfy the 
+[proper_fixed_equivocator_descriptors] property.
+*)
+Lemma not_equivocating_equivocatos_descriptors_proper_fixed
   (s : composite_state (equivocator_IM IM))
   (Hs : protocol_state_prop XE s)
-  (eqv_choice : equivocator_descriptors IM)
-  (Heqv_choice : not_equivocating_equivocator_descriptors IM eqv_choice s)
-  : proper_fixed_equivocator_descriptors eqv_choice s.
+  (eqv_descriptors : equivocator_descriptors IM)
+  (Heqv_descriptors : not_equivocating_equivocator_descriptors IM eqv_descriptors s)
+  : proper_fixed_equivocator_descriptors eqv_descriptors s.
 Proof.
-  apply not_equivocating_equivocator_descriptors_proper in Heqv_choice as Hproper.
+  apply not_equivocating_equivocator_descriptors_proper in Heqv_descriptors as Hproper.
   split; [assumption|].
   intros i Hi.
-  specialize (not_equivocating_equivocatos_choice_fixed_descriptor_is_0 _ Hs _ Hi)
+  specialize (not_equivocating_index_has_singleton_state _ Hs _ Hi)
     as Hzero.
   unfold is_singleton_state in Hzero.
-  specialize (Heqv_choice i). unfold not_equivocating_descriptor in Heqv_choice.
-  destruct (eqv_choice i); [contradiction|].
+  specialize (Heqv_descriptors i). unfold not_equivocating_descriptor in Heqv_descriptors.
+  destruct (eqv_descriptors i); [contradiction|].
   destruct b; [contradiction|].
   replace n with 0; [reflexivity|]. lia.
 Qed.
 
-Lemma proper_fixed_equivocator_descriptors_projection
+(**
+Projections of (valid) traces of the composition of equivocators preserve
+[proper_fixed_equivocator_descriptors].
+*)
+Lemma equivocators_trace_project_preserves_proper_fixed_equivocator_descriptors
   (is : composite_state (equivocator_IM IM))
   (tr : list (composite_transition_item (equivocator_IM IM)))
   (Htr : finite_protocol_trace_from (pre_loaded_with_all_messages_vlsm FreeE) is tr)
   (s := last (map destination tr) is)
-  (choice : equivocator_descriptors IM)
-  (ichoice : equivocator_descriptors IM)
+  (descriptors : equivocator_descriptors IM)
+  (idescriptors : equivocator_descriptors IM)
   (trX : list (composite_transition_item IM))
-  (HtrX : equivocators_trace_project IM choice tr = Some (trX, ichoice))
-  : proper_fixed_equivocator_descriptors choice s -> proper_fixed_equivocator_descriptors ichoice is.
+  (HtrX : equivocators_trace_project IM descriptors tr = Some (trX, idescriptors))
+  : proper_fixed_equivocator_descriptors descriptors s -> proper_fixed_equivocator_descriptors idescriptors is.
 Proof.
   intros [Hproper Hfixed].
   specialize
@@ -355,7 +432,7 @@ Proof.
   split; [assumption|].
   intros i Hi. specialize (Hfixed i Hi).
   revert Hfixed. clear Hi. revert i.
-  apply (not_equivocating_equivocatos_choice_fixed_descriptor_is_0_projection IM) with is tr trX
+  apply (equivocators_trace_project_preserves_zero_descriptors IM) with is tr trX
   ; assumption.
 Qed.
 
@@ -394,59 +471,67 @@ Qed.
 
 Existing Instance Free_has_been_observed_capability.
 Existing Instance Free_has_been_sent_capability.
+Existing Instance equivocating_i0.
 
-Definition constraint_prop
+(**
+This is a property of the [fixed_equivocation_constraint] which is being
+used to parameterize the [_equivocators_protocol_trace_project] lemma below
+allowing it to also be instantiated for the free composition.
+
+It basically says that if a message has_been_sent for a state of the 
+composition of equivocators with no-message equivocations and fixed
+state-equivocations, then any of its projections should be allowed to receive it.
+*)
+Definition constraint_has_been_sent_prop
   (constraint : composite_label IM -> composite_state IM * option message -> Prop)
   : Prop :=
   forall
-    (X' := composite_vlsm IM constraint)
-    (tr': list (composite_transition_item (equivocator_IM IM)))
-    (l: vlabel XE)
-    (input: message)
-    (is : _composite_state (equivocator_IM IM))
-    (Htr: finite_protocol_trace XE is tr')
-    (final_choice': equivocator_descriptors IM)
-    (trX': list (composite_transition_item IM))
-    (initial_choice: equivocator_descriptors IM)
-    (Htr_project: equivocators_trace_project IM final_choice' tr' = Some (trX', initial_choice))
-    (Hproper': proper_fixed_equivocator_descriptors final_choice' (last (map Common.destination tr') is))
-    (final_choice_m initial_choice_m: equivocator_descriptors IM)
-    (trXm: list (composite_transition_item IM))
-    (Hfinal_choice_m: proper_fixed_equivocator_descriptors final_choice_m (last (map Common.destination tr') is))
-    (Hproject_trXm: equivocators_trace_project IM final_choice_m tr' = Some (trXm, initial_choice_m))
-    (Hex: Exists (field_selector Common.output input) trXm),
-  constraint (existT (fun n : index => vlabel (IM n)) (projT1 l) (fst (projT2 l))) (last (map Common.destination trX') (equivocators_state_project IM initial_choice is), Some input).
+    (s : composite_state (equivocator_IM IM))
+    (Hs : protocol_state_prop XE s)
+    (descriptors : equivocator_descriptors IM)
+    (Hdescriptors : proper_fixed_equivocator_descriptors descriptors s)
+    (sX := @equivocators_state_project _ _ IndEqDec IM i0 descriptors s)
+    (m: message)
+    (Hinput : has_been_sent FreeE s m)
+    l,
+  constraint l (sX, Some m).
 
+(**
+Generic proof that the projection of a trace of the composition of equivocators
+with no message equivocation and fixed state equivocation is protocol w.r.t.
+the composition of the regular nodes constrained by a constraint satisfying
+several properties, including the [constraint_has_been_sent_prop]erty.
+*)
 Lemma _equivocators_protocol_trace_project
-  (final_choice : equivocator_descriptors IM)
+  (final_descriptors : equivocator_descriptors IM)
   (is : composite_state (equivocator_IM IM))
   (tr : list (composite_transition_item (equivocator_IM IM)))
   (final_state := last (map destination tr) is)
-  (Hproper : proper_fixed_equivocator_descriptors final_choice final_state)
+  (Hproper : proper_fixed_equivocator_descriptors final_descriptors final_state)
   (Htr : finite_protocol_trace XE is tr)
   (constraint : composite_label IM -> composite_state IM * option message -> Prop)
   (HconstraintNone : forall l s, constraint l (s, None))
   (Hconstraintinitial : forall l s m, vinitial_message_prop FreeE m -> constraint l (s, Some m))
-  (Hconstraint_noequiv :  constraint_prop constraint)
+  (Hconstraint_hbs :  constraint_has_been_sent_prop constraint)
   (X' := composite_vlsm IM constraint)
   : exists
     (trX : list (composite_transition_item IM))
-    (initial_choice : equivocator_descriptors IM)
-    (isX := equivocators_state_project IM initial_choice is)
+    (initial_descriptors : equivocator_descriptors IM)
+    (isX := equivocators_state_project IM initial_descriptors is)
     (final_stateX := last (map destination trX) isX),
-    proper_fixed_equivocator_descriptors initial_choice is /\
-    equivocators_trace_project IM final_choice tr = Some (trX, initial_choice) /\
-    equivocators_state_project IM final_choice final_state = final_stateX /\
+    proper_fixed_equivocator_descriptors initial_descriptors is /\
+    equivocators_trace_project IM final_descriptors tr = Some (trX, initial_descriptors) /\
+    equivocators_state_project IM final_descriptors final_state = final_stateX /\
     finite_protocol_trace X' isX trX.
 Proof.
   remember (length tr) as len_tr.
-  generalize dependent final_choice. generalize dependent tr.
+  generalize dependent final_descriptors. generalize dependent tr.
   induction len_tr using (well_founded_induction Wf_nat.lt_wf); intros.
   subst len_tr.
   destruct_list_last tr tr' lst Htr_lst.
-  - clear H. subst. unfold final_state in *. exists [], final_choice.
+  - clear H. subst. unfold final_state in *. exists [], final_descriptors.
     split; [assumption|]. split; [reflexivity|]. split; [reflexivity|].
-    remember (equivocators_state_project IM final_choice is) as isx.
+    remember (equivocators_state_project IM final_descriptors is) as isx.
     cut (vinitial_state_prop X' isx).
     { intro. split; [|assumption]. constructor.
       apply protocol_state_prop_iff. left.
@@ -461,14 +546,14 @@ Proof.
     apply finite_protocol_trace_from_app_iff in Htr.
     destruct Htr as [Htr Hlst].
     specialize (H' tr' (conj Htr Hinit) eq_refl).
-    specialize (equivocators_transition_item_project_proper_characterization IM final_choice lst) as Hproperx.
+    specialize (equivocators_transition_item_project_proper_characterization IM final_descriptors lst) as Hproperx.
     specialize
-      (equivocators_transition_item_project_zero_descriptor IM final_choice lst)
+      (equivocators_transition_item_project_preserves_zero_descriptors IM final_descriptors lst)
       as Hzero.
     unfold final_state in Hproper. rewrite Htr_lst in Hproper.
     rewrite map_app in Hproper. simpl in Hproper. rewrite last_is_last in Hproper.
     spec Hproperx (proj1 Hproper).
-    destruct Hproperx as [oitem [final_choice' [Hprojectx [Hitemx Hproperx]]]].
+    destruct Hproperx as [oitem [final_descriptors' [Hprojectx [Hitemx Hproperx]]]].
     specialize (Hproperx (last (map destination tr') is)).
     unfold equivocators_trace_project.
     rewrite fold_right_app.
@@ -479,17 +564,17 @@ Proof.
     rewrite Hprojectx in Heqfoldx.
     inversion Hlst. subst tl s' lst.
     destruct H4 as [[Hs [Hiom [Hv Hc]]] Ht].
-    specialize (Hzero oitem final_choice' _ Ht Hv Hprojectx).
+    specialize (Hzero oitem final_descriptors' _ Ht Hv Hprojectx).
     specialize (Hproperx Hv Ht).
     destruct Hproperx as [_Hproper' Hx].
-    assert (Hproper' : proper_fixed_equivocator_descriptors final_choice' (last (map destination tr') is)).
+    assert (Hproper' : proper_fixed_equivocator_descriptors final_descriptors' (last (map destination tr') is)).
     { split; [assumption|].
       intros i Hi. apply Hzero. clear Hzero. destruct Hproper as [_ Hzero].
       apply Hzero. assumption.
     }
     clear _Hproper' Hzero.
     specialize (H' _ Hproper').
-    destruct H' as [trX' [initial_choice [_ [Htr_project [Hstate_project HtrX']]]]].
+    destruct H' as [trX' [initial_descriptors [_ [Htr_project [Hstate_project HtrX']]]]].
     assert
       (Htr' : finite_protocol_trace FreeE is tr').
     {  split; [|assumption].
@@ -503,14 +588,14 @@ Proof.
       apply (VLSM_incl_finite_protocol_trace_from _ _ Hincl). apply Htr'.
     }
     specialize
-      (proper_fixed_equivocator_descriptors_projection _ _ (proj1 Htr'pre) _ _ _ Htr_project Hproper')
+      (equivocators_trace_project_preserves_proper_fixed_equivocator_descriptors _ _ (proj1 Htr'pre) _ _ _ Htr_project Hproper')
       as Hproper_initial.
     destruct oitem as [item|].
     +  simpl in Hitemx. destruct Hitemx as [Hl [Hinput [Houtput Hdestination]]].
       specialize (Hx _ eq_refl).
       destruct Hx as [Hvx Htx].
-      exists (trX' ++ [item]), initial_choice. subst foldx.
-      rewrite equivocators_trace_project_folder_additive with (trX := trX') (eqv_descriptors := initial_choice)
+      exists (trX' ++ [item]), initial_descriptors. subst foldx.
+      rewrite equivocators_trace_project_folder_additive with (trX := trX') (eqv_descriptors := initial_descriptors)
       ; [|assumption].
       split; [assumption|].
       split; [reflexivity|].
@@ -559,28 +644,29 @@ Proof.
       spec Hall Htr'.
       specialize (Hall eq_refl).
       destruct (equivocators_trace_project_output_reflecting_inv IM _ _ (proj1 Htr'pre) _ Hall)
-        as [final_choice_m [initial_choice_m [trXm [_Hfinal_choice_m [Hproject_trXm Hex]]]]].
-      assert (Hfinal_choice_m : proper_fixed_equivocator_descriptors final_choice_m (last (map Common.destination tr') is)).
-      { apply not_equivocating_equivocatos_choice_proper_fixed; [|assumption].
+        as [final_descriptors_m [initial_descriptors_m [trXm [_Hfinal_descriptors_m [Hproject_trXm Hex]]]]].
+      assert (Hfinal_descriptors_m : proper_fixed_equivocator_descriptors final_descriptors_m (last (map Common.destination tr') is)).
+      { apply not_equivocating_equivocatos_descriptors_proper_fixed; [|assumption].
         apply finite_ptrace_last_pstate. assumption.
       }
       specialize (H (length tr')).
       spec H. { rewrite app_length. simpl. lia. }
-      specialize (H tr' (conj Htr Hinit) eq_refl final_choice_m Hfinal_choice_m).
-      destruct H as [trXm' [initial_choice_m' [Hproper_initial_m [Hproject_trXm' [Hpr_fin_tr' HtrXm]]]]].
+      specialize (H tr' (conj Htr Hinit) eq_refl final_descriptors_m Hfinal_descriptors_m).
+      destruct H as [trXm' [initial_descriptors_m' [Hproper_initial_m [Hproject_trXm' [Hpr_fin_tr' HtrXm]]]]].
       simpl in *. rewrite Hproject_trXm in Hproject_trXm'.
-      inversion Hproject_trXm'. subst trXm' initial_choice_m'. clear Hproject_trXm'.
+      inversion Hproject_trXm'. subst trXm' initial_descriptors_m'. clear Hproject_trXm'.
       repeat split; [assumption| |assumption| |assumption]
       ; [ apply option_protocol_message_Some
         ; apply (protocol_trace_output_is_protocol X' _ _ (proj1 HtrXm) _ Hex)
         |].
-      apply
-        (Hconstraint_noequiv 
-          tr' l input is (conj Htr Hinit) final_choice' trX' initial_choice Htr_project
-          Hproper' final_choice_m initial_choice_m trXm Hfinal_choice_m
-          Hproject_trXm Hex
-        ).
-    + exists trX'. exists initial_choice. subst foldx. split; [assumption|].
+      rewrite <- Hstate_project.
+      apply Hconstraint_hbs; [assumption| apply Hproper'|].
+      assert (Hlst'pre : protocol_state_prop (pre_loaded_with_all_messages_vlsm FreeE) (last (map Common.destination tr') is)).
+      { apply finite_ptrace_last_pstate. apply Htr'pre. }
+      apply proper_sent; [assumption|].
+      apply has_been_sent_consistency; [assumption| assumption| ].
+      exists is, tr', Htr'pre, eq_refl. assumption.
+    + exists trX'. exists initial_descriptors. subst foldx. split; [assumption|].
       split; [apply Htr_project|]. split; [|assumption].
       subst tr. clear -Hstate_project Hx.
       rewrite Hstate_project in Hx.
@@ -588,25 +674,27 @@ Proof.
       rewrite map_app. simpl. rewrite last_is_last. reflexivity.
 Qed.
 
+(** Instantiating the lemma above with the free constraint.
+*)
 Lemma free_equivocators_protocol_trace_project
-  (final_choice : equivocator_descriptors IM)
+  (final_descriptors : equivocator_descriptors IM)
   (is : composite_state (equivocator_IM IM))
   (tr : list (composite_transition_item (equivocator_IM IM)))
   (final_state := last (map destination tr) is)
-  (Hproper : proper_fixed_equivocator_descriptors final_choice final_state)
+  (Hproper : proper_fixed_equivocator_descriptors final_descriptors final_state)
   (Htr : finite_protocol_trace XE is tr)
   : exists
     (trX : list (composite_transition_item IM))
-    (initial_choice : equivocator_descriptors IM)
-    (isX := equivocators_state_project IM initial_choice is)
+    (initial_descriptors : equivocator_descriptors IM)
+    (isX := equivocators_state_project IM initial_descriptors is)
     (final_stateX := last (map destination trX) isX),
-    proper_fixed_equivocator_descriptors initial_choice is /\
-    equivocators_trace_project IM final_choice tr = Some (trX, initial_choice) /\
-    equivocators_state_project IM final_choice final_state = final_stateX /\
+    proper_fixed_equivocator_descriptors initial_descriptors is /\
+    equivocators_trace_project IM final_descriptors tr = Some (trX, initial_descriptors) /\
+    equivocators_state_project IM final_descriptors final_state = final_stateX /\
     finite_protocol_trace (free_composite_vlsm IM) isX trX.
 Proof.
   apply _equivocators_protocol_trace_project; [assumption | assumption| ..]
-  ; unfold constraint_prop; intros; exact I.
+  ; unfold constraint_has_been_sent_prop; intros; exact I.
 Qed.
 
 Lemma equivocators_trace_sub_item_input_is_seeded_or_sub_previously_sent
@@ -614,21 +702,21 @@ Lemma equivocators_trace_sub_item_input_is_seeded_or_sub_previously_sent
   (tr : list (vtransition_item XE))
   (s := last (map destination tr) is)
   (Htr : finite_protocol_trace XE is tr)
-  (initial_choice final_choice: equivocator_descriptors IM)
-  (Hproper: proper_fixed_equivocator_descriptors final_choice s)
+  (initial_descriptors final_descriptors: equivocator_descriptors IM)
+  (Hproper: proper_fixed_equivocator_descriptors final_descriptors s)
   (trX: list (composite_transition_item IM))
-  (Htr_project: equivocators_trace_project IM final_choice tr = Some (trX, initial_choice))
-  (lst_trX := last (map Common.destination trX) (equivocators_state_project IM initial_choice is))
+  (Htr_project: equivocators_trace_project IM final_descriptors tr = Some (trX, initial_descriptors))
+  (lst_trX := last (map Common.destination trX) (equivocators_state_project IM initial_descriptors is))
   : trace_sub_item_input_is_seeded_or_sub_previously_sent 
     (equivocator_IM IM) equivocating
     (no_additional_equivocations (free_composite_vlsm IM) lst_trX) tr.
 Proof.
   intros pre item suf m Heq Hm Hitem.
-  destruct (free_equivocators_protocol_trace_project final_choice is tr Hproper Htr)
-    as [_trX [_initial_choice [Hinitial_choice [_Htr_project [Hfinal_state HtrXFree]]]]].
+  destruct (free_equivocators_protocol_trace_project final_descriptors is tr Hproper Htr)
+    as [_trX [_initial_descriptors [Hinitial_descriptors [_Htr_project [Hfinal_state HtrXFree]]]]].
   rewrite Htr_project in _Htr_project.
-  inversion _Htr_project. subst _trX _initial_choice. clear _Htr_project.
-  assert (HtrXPre : finite_protocol_trace (pre_loaded_with_all_messages_vlsm (free_composite_vlsm IM)) (equivocators_state_project IM initial_choice is) trX).
+  inversion _Htr_project. subst _trX _initial_descriptors. clear _Htr_project.
+  assert (HtrXPre : finite_protocol_trace (pre_loaded_with_all_messages_vlsm (free_composite_vlsm IM)) (equivocators_state_project IM initial_descriptors is) trX).
   { apply VLSM_incl_finite_protocol_trace with (machine (free_composite_vlsm IM)); [|apply HtrXFree].
     apply vlsm_incl_pre_loaded_with_all_messages_vlsm.
   }
@@ -688,9 +776,9 @@ Proof.
   rewrite has_been_observed_sent_received_iff; [|assumption].
   right. apply proper_sent; [assumption|].
   apply has_been_sent_consistency; [assumption| assumption |].
-  exists (equivocators_state_project IM initial_choice is), trX, HtrXPre, eq_refl.
+  exists (equivocators_state_project IM initial_descriptors is), trX, HtrXPre, eq_refl.
   apply equivocators_trace_project_app_iff in Htr_project.
-  destruct Htr_project as [preX [sufX [final_choice' [Hsuf_project [Htr_project Heq]]]]].
+  destruct Htr_project as [preX [sufX [final_descriptors' [Hsuf_project [Htr_project Heq]]]]].
 
   subst trX.
   apply Exists_app. left.
@@ -721,8 +809,8 @@ Proof.
   clear Hsuf_free Hpre_free.
   destruct Htr_free as [Hpre_free _]. apply finite_protocol_trace_from_app_iff in Hpre_free.
   destruct Hpre_free as [Hpre_free Hsuf_free].
-  assert (Hfinal' : forall i, ~In i equivocating -> final_choice' i = Existing _ 0 false).
-  { specialize (not_equivocating_equivocatos_choice_fixed_descriptor_is_0_projection IM _ _ Hsuf_free final_choice) as Hpr.
+  assert (Hfinal' : forall i, ~In i equivocating -> final_descriptors' i = Existing _ 0 false).
+  { specialize (equivocators_trace_project_preserves_zero_descriptors IM _ _ Hsuf_free final_descriptors) as Hpr.
     specialize (Hpr _ _ Hsuf_project).
     intros i Hi.
     apply Hpr. apply (proj2 Hproper). assumption.
@@ -738,27 +826,27 @@ Proof.
   subst pre.
 
   apply equivocators_trace_project_app_iff in Htr_project.
-  destruct Htr_project as [preX' [sufX' [eqv_choice' [Hpr_suf [Hpr_pre HpreX]]]]].
+  destruct Htr_project as [preX' [sufX' [eqv_descriptors' [Hpr_suf [Hpr_pre HpreX]]]]].
   subst preX. apply Exists_app. right.
 
   apply (finite_protocol_trace_from_app_iff (pre_loaded_with_all_messages_vlsm FreeE)) in Hpre_free.
   destruct Hpre_free as [Hpre'_free Hsuf'_free].
 
   apply equivocators_trace_project_app_iff in Hpr_suf.
-  destruct Hpr_suf as [pre_itemX [sufX'' [eqv_choice'' [Hpr_suf' [Hpr_pre_item HsufX']]]]].
+  destruct Hpr_suf as [pre_itemX [sufX'' [eqv_descriptors'' [Hpr_suf' [Hpr_pre_item HsufX']]]]].
   subst sufX'. apply Exists_app. left.
 
   apply (finite_protocol_trace_from_app_iff (pre_loaded_with_all_messages_vlsm FreeE)) in Hsuf'_free.
   destruct Hsuf'_free as [Hpre_item_free Hsuf'_free].
-  assert (Heqv_choice'' : forall i, ~In i equivocating -> eqv_choice'' i = Existing _ 0 false).
-  { specialize (not_equivocating_equivocatos_choice_fixed_descriptor_is_0_projection IM _ _ Hsuf'_free final_choice') as Hpr.
+  assert (Heqv_descriptors'' : forall i, ~In i equivocating -> eqv_descriptors'' i = Existing _ 0 false).
+  { specialize (equivocators_trace_project_preserves_zero_descriptors IM _ _ Hsuf'_free final_descriptors') as Hpr.
     specialize (Hpr _ _ Hpr_suf').
     intros i Hi.
     apply Hpr. apply Hfinal'. assumption.
   }
 
   assert (Hsingleton_d_pre_item : is_singleton_state (IM (projT1 (Common.l pre_item))) (destination pre_item (projT1 (Common.l pre_item)))).
-  { apply not_equivocating_equivocatos_choice_fixed_descriptor_is_0; [|assumption].
+  { apply not_equivocating_index_has_singleton_state; [|assumption].
     clear -Htr.
     apply finite_protocol_trace_from_app_iff in Htr.
     destruct Htr as [Htr _].
@@ -772,10 +860,10 @@ Proof.
   }
 
 
-  clear -Hpr_pre_item Heqv_choice'' Hpre_m n Hpre_item_free Hsingleton_d_pre_item.
-  specialize (Heqv_choice'' _ n).
+  clear -Hpr_pre_item Heqv_descriptors'' Hpre_m n Hpre_item_free Hsingleton_d_pre_item.
+  specialize (Heqv_descriptors'' _ n).
   simpl in *.
-  destruct (equivocators_transition_item_project IM eqv_choice'' pre_item)
+  destruct (equivocators_transition_item_project IM eqv_descriptors'' pre_item)
     as [(o, odescriptor)|] eqn:Hpr
   ; [|congruence].
   destruct pre_item. simpl in *.
@@ -795,7 +883,7 @@ Proof.
   unfold ProjectionTraces.composite_transition_item_projection_from_eq in Hpr.
   simpl in Hpr.
   unfold eq_rect_r in Hpr. simpl in Hpr.
-  rewrite Heqv_choice'' in Hpr.
+  rewrite Heqv_descriptors'' in Hpr.
   unfold equivocator_vlsm_transition_item_project in Hpr.
   rewrite state_update_eq in Hpr.
   destruct si' as (nsi', bsi').
@@ -817,11 +905,11 @@ Lemma equivocator_vlsm_trace_project_reflect_non_equivocating
   (tr': list (composite_transition_item (equivocator_IM IM)))
   (Htr': finite_protocol_trace XE is tr')
   (input: message)
-  (final_choice': equivocator_descriptors IM)
-  (Hproper': proper_fixed_equivocator_descriptors final_choice' (last (map destination tr') is))
+  (final_descriptors': equivocator_descriptors IM)
+  (Hproper': proper_fixed_equivocator_descriptors final_descriptors' (last (map destination tr') is))
   (trX': list (composite_transition_item IM))
-  (initial_choice: equivocator_descriptors IM)
-  (Htr_project: equivocators_trace_project IM final_choice' tr' = Some (trX', initial_choice))
+  (initial_descriptors: equivocator_descriptors IM)
+  (Htr_project: equivocators_trace_project IM final_descriptors' tr' = Some (trX', initial_descriptors))
   (item: composite_transition_item (equivocator_IM IM))
   (Hitem: In item tr')
   (Houtput: output item = Some input)
@@ -856,18 +944,18 @@ Proof.
     - apply vlsm_incl_pre_loaded_with_all_messages_vlsm.
   }
   specialize
-    (proper_fixed_equivocator_descriptors_projection _ _ Hsufpre
-      final_choice' eqv_item _ Hpr_suf Hproper'
+    (equivocators_trace_project_preserves_proper_fixed_equivocator_descriptors _ _ Hsufpre
+      final_descriptors' eqv_item _ Hpr_suf Hproper'
     ) as Hproper_item.
   destruct Hproper_item as [Hproper_item Hproper_fixed_item].
   specialize (Hproper_fixed_item _ Hno_equiv_item).
   specialize
-    (equivocators_transition_item_project_zero_descriptor_no_equivocation IM eqv_item item
+    (no_equivocating_equivocators_transition_item_project IM eqv_item item
       Hproper_fixed_item
     ) as Hex.
   spec Hex.
   {
-    apply not_equivocating_equivocatos_choice_fixed_descriptor_is_0; [|assumption].
+    apply not_equivocating_index_has_singleton_state; [|assumption].
     apply finite_ptrace_last_pstate in Hitem. assumption.
   }
   inversion Hitem; subst. destruct H3 as [[Hs [Hiom [Hv Hc]]] Ht].
@@ -881,20 +969,20 @@ Lemma has_not_been_observed_piecewise
   (is: _composite_state (equivocator_IM IM))
   (tr': list (composite_transition_item (equivocator_IM IM)))
   (Htr': finite_protocol_trace XE is tr')
-  (final_choice': equivocator_descriptors IM)
-  (Hproper': proper_fixed_equivocator_descriptors final_choice' (last (map destination tr') is))
+  (final_descriptors': equivocator_descriptors IM)
+  (Hproper': proper_fixed_equivocator_descriptors final_descriptors' (last (map destination tr') is))
   (trX': list (composite_transition_item IM))
-  (initial_choice: equivocator_descriptors IM)
-  (Htr_project: equivocators_trace_project IM final_choice' tr' = Some (trX', initial_choice))
+  (initial_descriptors: equivocator_descriptors IM)
+  (Htr_project: equivocators_trace_project IM final_descriptors' tr' = Some (trX', initial_descriptors))
   (input: message)
-  (Hno: ~ has_been_observed Free (last (map destination trX') (equivocators_state_project IM initial_choice is)) input)
+  (Hno: ~ has_been_observed Free (last (map destination trX') (equivocators_state_project IM initial_descriptors is)) input)
   : forall item : composite_transition_item (equivocator_IM IM),
       In item tr' -> output item = Some input -> In (projT1 (l item)) equivocating.
 Proof.
-  destruct (free_equivocators_protocol_trace_project final_choice' is tr' Hproper' Htr')
-    as [_trX' [_initial_choice [_ [_Htr_project [_ HtrX']]]]].
+  destruct (free_equivocators_protocol_trace_project final_descriptors' is tr' Hproper' Htr')
+    as [_trX' [_initial_descriptors [_ [_Htr_project [_ HtrX']]]]].
   rewrite Htr_project in _Htr_project.
-  inversion _Htr_project. subst _trX' _initial_choice. clear _Htr_project.
+  inversion _Htr_project. subst _trX' _initial_descriptors. clear _Htr_project.
   intros item Hitem Houtput.
   destruct (in_dec IndEqDec (projT1 (l item)) equivocating); [assumption|].
   elim Hno. clear Hno.
@@ -904,7 +992,7 @@ Proof.
       Free_has_been_sent_capability
       Free_has_been_observed_capability
     ) as Hsent_received.
-  assert (HtrX'_free : finite_protocol_trace (pre_loaded_with_all_messages_vlsm Free) (equivocators_state_project IM initial_choice is) trX').
+  assert (HtrX'_free : finite_protocol_trace (pre_loaded_with_all_messages_vlsm Free) (equivocators_state_project IM initial_descriptors is) trX').
   {
     revert HtrX'. clear. apply VLSM_incl_finite_protocol_trace.
     apply vlsm_incl_pre_loaded_with_all_messages_vlsm.
@@ -914,197 +1002,223 @@ Proof.
   apply Hsent_received. clear Hsent_received. right.
   apply proper_sent; [assumption|].
   apply has_been_sent_consistency; [assumption| assumption |].
-  exists (equivocators_state_project IM initial_choice is), trX', HtrX'_free, eq_refl.
+  exists (equivocators_state_project IM initial_descriptors is), trX', HtrX'_free, eq_refl.
   clear HtrX' HtrX'_free Hfree_lst.
-  apply equivocator_vlsm_trace_project_reflect_non_equivocating with is tr' final_choice' initial_choice item
+  apply equivocator_vlsm_trace_project_reflect_non_equivocating with is tr' final_descriptors' initial_descriptors item
   ; assumption.
 Qed.
 
-Lemma fixed_equivocators_protocol_trace_project
-  (final_choice : equivocator_descriptors IM)
+Lemma fixed_equivocation_constraint_has_constraint_has_been_sent_prop
+  : constraint_has_been_sent_prop
+    (fixed_equivocation_constraint IM Hbs Hbr equivocating Hi0_equiv finite_index).
+Proof.
+  unfold constraint_has_been_sent_prop. intros.
+  match goal with
+  |- fixed_equivocation_constraint _ _ _ _ _ _ _ (?l, _) => remember l as sX
+  end.
+  destruct (Free_no_additional_equivocation_decidable sX m)
+  ; [left; assumption|right].
+  exists m. split; [reflexivity|].
+  unfold no_additional_equivocations in n.
+  match type of n with
+  | ~ (?o \/ ?i) => assert (Hn : ~ o /\ ~ i) by intuition
+  end.
+  clear n; destruct Hn as [Hno Hni].
+  apply protocol_state_has_trace in Hs.
+  destruct Hs as [is [tr [Htr Heqs]]]. subst s.
+
+  assert (Htr'pre : finite_protocol_trace (pre_loaded_with_all_messages_vlsm FreeE) is tr).
+  { revert Htr. apply VLSM_incl_finite_protocol_trace.
+    apply VLSM_incl_trans with (machine FreeE).
+    - apply
+      (constraint_free_incl (equivocator_IM IM) (equivocators_fixed_equivocations_constraint IM Hbs
+        finite_index equivocating Hi0_equiv)).
+    - apply vlsm_incl_pre_loaded_with_all_messages_vlsm.
+  }
+
+  destruct
+    (preloaded_equivocators_protocol_trace_from_project IM
+      descriptors is tr (proj1 Hdescriptors) (proj1 Htr'pre)
+    )
+    as [trX [initial_descriptors [Htr_project [_ Hlst]]]].
+  simpl in Hlst, HeqsX.
+  rewrite Hlst in  HeqsX.
+  specialize 
+    (equivocators_trace_sub_item_input_is_seeded_or_sub_previously_sent
+      _ _ Htr initial_descriptors descriptors Hdescriptors _ Htr_project
+    ) as Hsub.
+  specialize
+    (finite_protocol_trace_sub_projection (equivocator_IM IM) equivocating Hi0_equiv
+      (equivocators_fixed_equivocations_constraint IM Hbs finite_index equivocating Hi0_equiv)
+      (equivocator_Hbs IM Hbs)
+      finite_index
+      (no_additional_equivocations (free_composite_vlsm IM) sX)
+    ) as Hproject.
+  spec Hproject.
+  { intros l' (s', om').
+    unfold equivocators_fixed_equivocations_constraint.
+    unfold equivocators_no_equivocations_constraint.
+    unfold no_equivocations_additional_constraint.
+    clear. intuition.
+  }
+  spec Hproject is tr.
+  spec Hproject. { subst sX. assumption. }
+  spec Hproject Htr.
+  clear Hsub.
+  subst sX.
+  unfold pre_loaded_free_equivocating_vlsm_composition.
+  assert (Hplst : protocol_state_prop (pre_loaded_with_all_messages_vlsm FreeE) (last (map destination tr) is)).
+  { apply (finite_ptrace_last_pstate (pre_loaded_with_all_messages_vlsm FreeE)).
+    apply Htr'pre.
+  }
+  apply proper_sent in Hinput; [|assumption].
+  specialize (Hinput is tr Htr'pre eq_refl).
+  apply (equivocators_trace_project_output_reflecting_iff _ _ _ (proj1 Htr'pre)) in Hinput.
+  destruct Hinput as [final_descriptors_m [initial_descriptors_m [trXm [Hfinal_descriptors_m [Hproject_trXm Hex]]]]].
+  specialize
+    (seeded_equivocators_protocol_trace_project (sub_IM IM equivocating)
+      (sub_has_been_sent_capabilities IM equivocating Hbs)
+      (finite_sub_index equivocating finite_index)
+      (fun m : message =>
+        no_additional_equivocations (free_composite_vlsm IM)
+          (last (map Common.destination trX)
+             (equivocators_state_project IM initial_descriptors is)) m \/
+        vinitial_message_prop (free_composite_vlsm IM) m)
+      (fun i => final_descriptors_m (proj1_sig i))
+      (composite_state_sub_projection (equivocator_IM IM) equivocating is)
+      (finite_trace_sub_projection (equivocator_IM IM) equivocating tr)
+    ) as Hsub_project.
+  simpl in Hsub_project.
+  spec Hsub_project.
+  { specialize (preloaded_finite_trace_sub_projection_last_state (equivocator_IM IM) equivocating Hi0_equiv _ _ (proj1 Htr'pre))
+      as Heq_lst.
+    simpl in Heq_lst.
+    match goal with
+    |- proper_equivocator_descriptors _ _ ?l =>
+      match type of Heq_lst with
+      | _ = ?l' =>
+        replace l with l'
+      end
+    end.
+    intros e.
+    destruct e. simpl.
+    unfold sub_IM. unfold composite_state_sub_projection. simpl.
+    apply not_equivocating_equivocator_descriptors_proper in Hfinal_descriptors_m.
+    apply Hfinal_descriptors_m.
+  }
+  spec Hsub_project.
+  { clear -Hproject.
+    unfold seeded_equivocators_no_equivocation_vlsm.
+    destruct Hproject as [Hproject Hinit].
+    split; [|assumption].
+    eapply VLSM_incl_finite_protocol_trace_from; [|apply Hproject].
+    unfold composite_vlsm.
+    unfold mk_vlsm. unfold projT2.
+    match goal with
+    |- VLSM_incl_part ?MX ?MY =>
+      apply (basic_VLSM_incl MX MY)
+    end
+    ; intros; [assumption | .. | reflexivity].
+    - apply initial_message_is_protocol.
+      simpl.
+      destruct H0; [|right; left; assumption].
+      simpl in H0. left. assumption.
+    - destruct H as [Hs [_ [Hv Hc]]].
+      split; [assumption|].
+      destruct Hc as [Hc _].
+      split; [|exact I].
+      destruct om; [| exact I].
+      simpl in Hc. simpl.
+      destruct Hc as [Hc | [Hc | Hc]]
+      ; [| right; left; assumption| right; right; left; assumption].
+      left.
+      destruct Hc as [subi Hibs].
+      exists subi. revert Hibs.
+      apply has_been_sent_irrelevance.
+
+      match type of Hs with
+      | context [composite_vlsm_machine ?IM ?constraint] =>
+        apply (preloaded_protocol_state_projection IM constraint)
+      end.
+      revert Hs.
+      apply VLSM_incl_protocol_state.
+      apply pre_loaded_vlsm_incl_pre_loaded_with_all_messages.
+  }
+  destruct Hsub_project
+    as [trX' [initial_descriptors' [Hinitial_descriptors' [Hpr_tr' [Hpr_lst_tr' HtrX]]]]].
+  specialize
+    (has_not_been_observed_piecewise _ _ Htr
+      _ Hdescriptors
+      _ _ Htr_project
+      _ Hno
+    ) as Hno'.
+  destruct
+    (equivocators_trace_project_finite_trace_sub_projection_commute IM equivocating Hi0_equiv
+      final_descriptors_m initial_descriptors_m initial_descriptors' tr trXm trX'
+      Hproject_trXm Hpr_tr'
+    )
+    as [_ HeqtrX].
+  remember
+    (equivocators_state_project (sub_IM IM equivocating) initial_descriptors'
+      (composite_state_sub_projection (equivocator_IM IM) equivocating is)
+    ) as isX.
+  clear - HeqtrX HtrX Hno' Hex Hproject_trXm (* Htr'pre Hfinal_descriptors_m *).
+  apply can_emit_from_protocol_trace with isX trX'; [assumption|].
+
+  apply Exists_exists in Hex.
+  destruct Hex as [output_itemX [Hin Houtput_select]].
+  apply in_split in Hin.
+  destruct Hin as [preX [sufX Heq_trXm]].
+  change (output_itemX :: sufX) with ([output_itemX] ++ sufX) in Heq_trXm.
+  subst trXm.
+  apply equivocators_trace_project_app_inv_item in Hproject_trXm.
+  destruct Hproject_trXm as [pre [suf [item [item_descriptors [pre_descriptors [Hpr_suf [Hpr_item [Hpr_pre Heqtr]]]]]]]].
+  subst.
+
+  specialize (Hno' item).
+  spec Hno'.
+  { rewrite !in_app_iff. right. left. left. reflexivity. }
+  rewrite! (finite_trace_sub_projection_app IM).
+  unfold trace_has_message.
+  rewrite! Exists_app. right. left. simpl.
+
+  unfold equivocators_transition_item_project in Hpr_item.
+  destruct
+    (equivocator_vlsm_transition_item_project (IM (projT1 (l item)))
+      (composite_transition_item_projection (equivocator_IM IM) item)
+      (item_descriptors (projT1 (l item)))
+    ) as [(o, deqv')|] eqn:Hpr_itemi
+    ; [|congruence].
+  destruct o as [item'|]; [|congruence].
+  inversion Hpr_item. subst. spec Hno' Houtput_select.
+  unfold from_sub_projection. simpl.
+  destruct (decide (sub_index_prop equivocating (projT1 (l item))))
+  ; [|contradiction].
+  constructor. simpl. assumption.
+Qed.
+
+Theorem fixed_equivocators_protocol_trace_project
+  (final_descriptors : equivocator_descriptors IM)
   (is : composite_state (equivocator_IM IM))
   (tr : list (composite_transition_item (equivocator_IM IM)))
   (final_state := last (map destination tr) is)
-  (Hproper: proper_fixed_equivocator_descriptors final_choice final_state)
+  (Hproper: proper_fixed_equivocator_descriptors final_descriptors final_state)
   (Htr : finite_protocol_trace XE is tr)
   : exists
     (trX : list (composite_transition_item IM))
-    (initial_choice : equivocator_descriptors IM)
-    (isX := equivocators_state_project IM initial_choice is)
+    (initial_descriptors : equivocator_descriptors IM)
+    (isX := equivocators_state_project IM initial_descriptors is)
     (final_stateX := last (map destination trX) isX),
-    proper_fixed_equivocator_descriptors initial_choice is /\
-    equivocators_trace_project IM final_choice tr = Some (trX, initial_choice) /\
-    equivocators_state_project IM final_choice final_state = final_stateX /\
+    proper_fixed_equivocator_descriptors initial_descriptors is /\
+    equivocators_trace_project IM final_descriptors tr = Some (trX, initial_descriptors) /\
+    equivocators_state_project IM final_descriptors final_state = final_stateX /\
     finite_protocol_trace X isX trX.
 Proof.
   apply _equivocators_protocol_trace_project; [assumption | assumption| ..]
   ; intros.
   - left. exact I.
   - left. right. assumption.
-  - clear final_choice is tr final_state Hproper Htr.
-    unfold constraint_prop. intros.
-    assert (Htr'pre : finite_protocol_trace (pre_loaded_with_all_messages_vlsm FreeE) is tr').
-    { revert Htr. apply VLSM_incl_finite_protocol_trace.
-      apply VLSM_incl_trans with (machine FreeE).
-      - apply
-        (constraint_free_incl (equivocator_IM IM) (equivocators_fixed_equivocations_constraint IM Hbs
-          finite_index equivocating Hi0_equiv)).
-      - apply vlsm_incl_pre_loaded_with_all_messages_vlsm.
-    }
-    match goal with
-    |- fixed_equivocation_constraint _ _ _ _ _ _ _ (?l, _) => remember l as lst_trX
-    end.
-    destruct (Free_no_additional_equivocation_decidable lst_trX input)
-    ; [left; assumption|right].
-    exists input. split; [reflexivity|].
-    unfold no_additional_equivocations in n.
-    match type of n with
-    | ~ (?o \/ ?i) => assert (Hn : ~ o /\ ~ i) by intuition
-    end.
-    clear n; destruct Hn as [Hno Hni].
-    specialize 
-      (equivocators_trace_sub_item_input_is_seeded_or_sub_previously_sent
-        _ _ Htr initial_choice final_choice' Hproper' _ Htr_project
-      ) as Hsub.
-    specialize
-      (finite_protocol_trace_sub_projection (equivocator_IM IM) equivocating Hi0_equiv
-        (equivocators_fixed_equivocations_constraint IM Hbs finite_index equivocating Hi0_equiv)
-        (equivocator_Hbs IM Hbs)
-        finite_index
-        (no_additional_equivocations (free_composite_vlsm IM) lst_trX)
-      ) as Hproject.
-    spec Hproject.
-    { intros l' (s', om').
-      unfold equivocators_fixed_equivocations_constraint.
-      unfold equivocators_no_equivocations_constraint.
-      unfold no_equivocations_additional_constraint.
-      clear. intuition.
-    }
-    spec Hproject is tr'.
-    spec Hproject. { subst lst_trX. assumption. }
-    spec Hproject Htr.
-    clear Hsub.
-    subst lst_trX.
-    unfold seeded_free_equivocators_composition.
-    specialize
-      (seeded_equivocators_protocol_trace_project (sub_IM IM equivocating)
-        (sub_has_been_sent_capabilities IM equivocating Hbs)
-        (finite_sub_index equivocating finite_index)
-        (fun m : message =>
-          no_additional_equivocations (free_composite_vlsm IM)
-            (last (map Common.destination trX')
-               (equivocators_state_project IM initial_choice is)) m \/
-          vinitial_message_prop (free_composite_vlsm IM) m)
-        (fun i => final_choice_m (proj1_sig i))
-        (composite_state_sub_projection (equivocator_IM IM) equivocating is)
-        (finite_trace_sub_projection (equivocator_IM IM) equivocating tr')
-      ) as Hsub_project.
-    simpl in Hsub_project.
-    spec Hsub_project.
-    { specialize (preloaded_finite_trace_sub_projection_last_state (equivocator_IM IM) equivocating Hi0_equiv _ _ (proj1 Htr'pre))
-        as Heq_lst.
-      simpl in Heq_lst.
-      match goal with
-      |- proper_equivocator_descriptors _ _ ?l =>
-        match type of Heq_lst with
-        | _ = ?l' =>
-          replace l with l'
-        end
-      end.
-      intros e.
-      destruct e. simpl.
-      unfold sub_IM. unfold composite_state_sub_projection. simpl.
-      apply (proj1 Hfinal_choice_m).
-    }
-    spec Hsub_project.
-    { clear -Hproject.
-      unfold seeded_equivocators_no_equivocation_vlsm.
-      destruct Hproject as [Hproject Hinit].
-      split; [|assumption].
-      eapply VLSM_incl_finite_protocol_trace_from; [|apply Hproject].
-      unfold composite_vlsm.
-      unfold mk_vlsm. unfold projT2.
-      match goal with
-      |- VLSM_incl_part ?MX ?MY =>
-        apply (basic_VLSM_incl MX MY)
-      end
-      ; intros; [assumption | .. | reflexivity].
-      - apply initial_message_is_protocol.
-        simpl.
-        destruct H0; [|right; left; assumption].
-        simpl in H0. left. assumption.
-      - destruct H as [Hs [_ [Hv Hc]]].
-        split; [assumption|].
-        destruct Hc as [Hc _].
-        split; [|exact I].
-        destruct om; [| exact I].
-        simpl in Hc. simpl.
-        destruct Hc as [Hc | [Hc | Hc]]
-        ; [| right; left; assumption| right; right; left; assumption].
-        left.
-        destruct Hc as [subi Hibs].
-        exists subi. revert Hibs.
-        apply has_been_sent_irrelevance.
-
-        match type of Hs with
-        | context [composite_vlsm_machine ?IM ?constraint] =>
-          apply (preloaded_protocol_state_projection IM constraint)
-        end.
-        revert Hs.
-        apply VLSM_incl_protocol_state.
-        apply pre_loaded_vlsm_incl_pre_loaded_with_all_messages.
-    }
-    destruct Hsub_project
-      as [trX [initial_choice' [Hinitial_choice' [Hpr_tr' [Hpr_lst_tr' HtrX]]]]].
-    specialize
-      (has_not_been_observed_piecewise _ _ Htr
-        _ Hproper'
-        _ _ Htr_project
-        _ Hno
-      ) as Hno'.
-    destruct
-      (equivocators_trace_project_finite_trace_sub_projection_commute IM equivocating Hi0_equiv
-        final_choice_m initial_choice_m initial_choice' tr' trXm trX
-        Hproject_trXm Hpr_tr'
-      )
-      as [_ HeqtrX].
-    remember
-      (equivocators_state_project (sub_IM IM equivocating) initial_choice'
-        (composite_state_sub_projection (equivocator_IM IM) equivocating is)
-      ) as isX.
-    clear - HeqtrX HtrX Hno' Hex Hproject_trXm (* Htr'pre Hfinal_choice_m *).
-    apply can_emit_from_protocol_trace with isX trX; [assumption|].
-
-    apply Exists_exists in Hex.
-    destruct Hex as [output_itemX [Hin Houtput_select]].
-    apply in_split in Hin.
-    destruct Hin as [preX [sufX Heq_trXm]].
-    change (output_itemX :: sufX) with ([output_itemX] ++ sufX) in Heq_trXm.
-    subst trXm.
-    apply equivocators_trace_project_app_inv_item in Hproject_trXm.
-    destruct Hproject_trXm as [pre [suf [item [item_descriptors [pre_descriptors [Hpr_suf [Hpr_item [Hpr_pre Heqtr]]]]]]]].
-    subst.
-
-    specialize (Hno' item).
-    spec Hno'.
-    { rewrite !in_app_iff. right. left. left. reflexivity. }
-    rewrite! (finite_trace_sub_projection_app IM).
-    unfold trace_has_message.
-    rewrite! Exists_app. right. left. simpl.
-
-    unfold equivocators_transition_item_project in Hpr_item.
-    destruct
-      (equivocator_vlsm_transition_item_project (IM (projT1 (l item)))
-        (composite_transition_item_projection (equivocator_IM IM) item)
-        (item_descriptors (projT1 (l item)))
-      ) as [(o, deqv')|] eqn:Hpr_itemi
-      ; [|congruence].
-    destruct o as [item'|]; [|congruence].
-    inversion Hpr_item. subst. spec Hno' Houtput_select.
-    unfold from_sub_projection. simpl.
-    destruct (decide (sub_index_prop equivocating (projT1 (l item))))
-    ; [|contradiction].
-    constructor. simpl. assumption.
+  - apply fixed_equivocation_constraint_has_constraint_has_been_sent_prop.
 Qed.
 
 End from_equivocators_to_nodes.
