VLSM/Equivocators/Composition/Projections.v
@@ -64,15 +64,19 @@ Definition equivocators_transition_item_project
   | None => None
   end.
 
-Lemma equivocators_transition_item_project_zero_descriptor
-  (choice : equivocator_descriptors)
+(**
+[zero_descriptor]s are preserved when projecting [transition_item]s of the
+composition of equivocators.
+*)
+Lemma equivocators_transition_item_project_preserves_zero_descriptors
+  (descriptors : equivocator_descriptors)
   (item : composite_transition_item equivocator_IM)
-  oitem ichoice
+  oitem idescriptors
   s
   (Ht : composite_transition equivocator_IM (l item) (s, input item) = (destination item, output item))
   (Hv : composite_valid equivocator_IM (l item) (s, input item))
-  (Hpr : equivocators_transition_item_project choice item = Some (oitem, ichoice))
-  : forall i, choice i = Existing _ 0 false -> ichoice i = Existing _ 0 false.
+  (Hpr : equivocators_transition_item_project descriptors item = Some (oitem, idescriptors))
+  : forall i, descriptors i = Existing _ 0 false -> idescriptors i = Existing _ 0 false.
 Proof.
   intros i Hi.
   unfold equivocators_transition_item_project in Hpr.
@@ -114,7 +118,7 @@ Proof.
   destruct
     (equivocator_vlsm_transition_item_project (IM (projT1 (l item)))
       (composite_transition_item_projection equivocator_IM item)
-      (choice (projT1 (l item))))
+      (descriptors (projT1 (l item))))
     eqn: Hpr'; [|congruence].
   destruct p.
   destruct o; inversion Hpr
@@ -152,7 +156,11 @@ Proof.
   apply Hproper.
 Qed.
 
-Lemma equivocators_transition_item_project_zero_descriptor_no_equivocation
+(**
+A generalization of [no_equivocating_equivocator_transition_item_project] to
+the composition of equivocators.
+*)
+Lemma no_equivocating_equivocators_transition_item_project
   (eqv_descriptors : equivocator_descriptors)
   (item : composite_transition_item equivocator_IM)
   (i := projT1 (l item))
@@ -335,6 +343,30 @@ Proof.
     apply Hproper.
 Qed.
 
+Lemma equivocators_transition_item_project_inv_characterization
+  (eqv_descriptors eqv_descriptors': equivocator_descriptors)
+  (item : composite_transition_item equivocator_IM)
+  (itemx : composite_transition_item IM)
+  (Hpr_item : equivocators_transition_item_project eqv_descriptors item = Some (Some itemx, eqv_descriptors'))
+  : existT _ (projT1 (l item)) (fst (projT2 (l item))) = l itemx /\
+    input item = input itemx /\ output item = output itemx /\
+    equivocators_state_project eqv_descriptors (destination item) = destination itemx.
+Proof.
+  unfold equivocators_transition_item_project in Hpr_item.
+  destruct
+    (equivocator_vlsm_transition_item_project 
+      (IM (projT1 (l item)))
+      (composite_transition_item_projection equivocator_IM item)
+      (eqv_descriptors (projT1 (l item))))
+    as [([itemi|], descriptori)|] eqn:Hpr_itemi
+  ; [|congruence|congruence].
+  inversion Hpr_item. subst. clear Hpr_item. simpl.
+  repeat split.
+  apply equivocator_transition_item_project_inv_characterization in Hpr_itemi.
+  destruct Hpr_itemi as [Hl _].
+  rewrite Hl. reflexivity.
+Qed.
+
 Definition equivocators_trace_project_folder
   (item : composite_transition_item equivocator_IM)
   (result: option (list (composite_transition_item IM) * equivocator_descriptors))
@@ -465,7 +497,13 @@ Proof.
     exists preX. inversion Heq. subst _sufX _eqv_descriptors'.
     split; assumption.
 Qed.
- 
+
+(**
+For every [transition_item] of the projection of a trace over the composition
+of equivocators, there exists a corresponding item in the original trace
+which projects to it.
+
+*)
 Lemma equivocators_trace_project_app_inv_item
   (tr : list (composite_transition_item equivocator_IM))
   (ieqv_descriptors eqv_descriptors : equivocator_descriptors)
@@ -525,6 +563,9 @@ Proof.
         simpl. rewrite Hpr_x_item. reflexivity.
 Qed.
 
+(**
+A corrollary of the above, reflecting a split in the projection to the original trace.
+*)
 Lemma equivocators_trace_project_app_inv
   (tr : list (composite_transition_item equivocator_IM))
   (ieqv_descriptors eqv_descriptors : equivocator_descriptors)
@@ -553,25 +594,31 @@ Proof.
     simpl. rewrite Hpr_item. reflexivity.
 Qed.
 
+(**
+We can project a trace over the composition of equivocators in two ways:
+(1) first project on a equivocator component, then project the equivocator to the original component
+(2) first projects to the composition of original components, then project to one of them
 
+The result below says that the two ways lead to the same result.
+*)
 Lemma equivocators_trace_project_finite_trace_projection_list_commute
   (i : index)
-  (final_choice initial_choice : equivocator_descriptors)
+  (final_descriptors initial_descriptors : equivocator_descriptors)
   (eqv_initial : MachineDescriptor (IM i))
   (tr : list (composite_transition_item equivocator_IM))
   (trX : list (composite_transition_item IM))
   (trXi : list (vtransition_item (IM i)))
-  (eqv_final := final_choice i)
-  (Hproject_tr : equivocators_trace_project final_choice tr = Some (trX, initial_choice))
+  (eqv_final := final_descriptors i)
+  (Hproject_tr : equivocators_trace_project final_descriptors tr = Some (trX, initial_descriptors))
   (Hproject_tri :
     equivocator_vlsm_trace_project (IM i)
       (finite_trace_projection_list equivocator_IM i tr) eqv_final
     = Some (trXi, eqv_initial))
-  : initial_choice i = eqv_initial /\
+  : initial_descriptors i = eqv_initial /\
     finite_trace_projection_list IM i trX = trXi.
 Proof.
   generalize dependent trXi. generalize dependent trX.
-  generalize dependent final_choice.
+  generalize dependent final_descriptors.
   induction tr using rev_ind; intros.
   - simpl in Hproject_tr. inversion Hproject_tr. subst.
     clear Hproject_tr.
@@ -580,7 +627,7 @@ Proof.
   - unfold equivocators_trace_project in Hproject_tr.
     rewrite fold_right_app in Hproject_tr.
     match type of Hproject_tr with
-    | fold_right _ ?i _ = _ => destruct i as [(projectx,final_choice')|] eqn:Hproject_x
+    | fold_right _ ?i _ = _ => destruct i as [(projectx,final_descriptors')|] eqn:Hproject_x
     end
     ; [|rewrite equivocators_trace_project_fold_None in Hproject_tr; inversion Hproject_tr].
     apply equivocators_trace_project_folder_additive_iff in Hproject_tr.
@@ -589,10 +636,10 @@ Proof.
     rewrite finite_trace_projection_list_app in Hproject_tri.
     apply equivocator_vlsm_trace_project_app in Hproject_tri.
     destruct Hproject_tri as [eqv_final' [trXi' [project_xi [HtrXi' [Hproject_xi HeqtrXi]]]]].
-    assert (Hfinal'i : final_choice' i = eqv_final' /\ finite_trace_projection_list IM i projectx = project_xi).
+    assert (Hfinal'i : final_descriptors' i = eqv_final' /\ finite_trace_projection_list IM i projectx = project_xi).
     { clear - Hproject_x Hproject_xi.
       simpl in *.
-      destruct (equivocators_transition_item_project final_choice x)
+      destruct (equivocators_transition_item_project final_descriptors x)
         as [(ox, final')|] eqn:Hpr_item_x
       ; [|congruence].
       unfold equivocators_transition_item_project in Hpr_item_x.
@@ -601,7 +648,7 @@ Proof.
       - subst i. simpl in Hproject_xi.
         unfold eqv_final in *.
         remember
-          (equivocator_vlsm_transition_item_project (IM (projT1 (l x))) (composite_transition_item_projection_from_eq equivocator_IM x (projT1 (l x)) eq_refl) (final_choice (projT1 (l x))))
+          (equivocator_vlsm_transition_item_project (IM (projT1 (l x))) (composite_transition_item_projection_from_eq equivocator_IM x (projT1 (l x)) eq_refl) (final_descriptors (projT1 (l x))))
           as pr_item_x.
         destruct pr_item_x as [(oitem', descriptor')|]; [|discriminate Hproject_xi].
         destruct oitem' as [item'|]
@@ -627,7 +674,7 @@ Proof.
         unfold eqv_final in *.
         inversion Hproject_xi. subst. clear Hproject_xi.
         remember
-          (equivocator_vlsm_transition_item_project (IM (projT1 (l x))) (composite_transition_item_projection_from_eq equivocator_IM x (projT1 (l x)) eq_refl) (final_choice (projT1 (l x))))
+          (equivocator_vlsm_transition_item_project (IM (projT1 (l x))) (composite_transition_item_projection_from_eq equivocator_IM x (projT1 (l x)) eq_refl) (final_descriptors (projT1 (l x))))
           as pr_item_x.
         destruct pr_item_x as [(oitem', descriptor')|]; [|discriminate Hpr_item_x].
         destruct oitem' as [item'|]
@@ -675,28 +722,32 @@ Proof.
   apply seeded_equivocators_incl_preloaded.
 Qed.
 
-Lemma not_equivocating_equivocatos_choice_fixed_descriptor_is_0_projection
+(**
+A generalization of [equivocators_transition_item_project_preserves_zero_descriptors]
+to full (valid) traces
+*)
+Lemma equivocators_trace_project_preserves_zero_descriptors
   (is : composite_state equivocator_IM)
   (tr : list (composite_transition_item equivocator_IM))
   (Htr : finite_protocol_trace_from PreFreeE is tr)
   (s := last (map destination tr) is)
-  (choice : equivocator_descriptors)
-  (ichoice : equivocator_descriptors)
+  (descriptors : equivocator_descriptors)
+  (idescriptors : equivocator_descriptors)
   (trX : list (composite_transition_item IM))
-  (HtrX : equivocators_trace_project choice tr = Some (trX, ichoice))
-  : forall i, choice i = Existing _ 0 false -> ichoice i = Existing _ 0 false.
+  (HtrX : equivocators_trace_project descriptors tr = Some (trX, idescriptors))
+  : forall i, descriptors i = Existing _ 0 false -> idescriptors i = Existing _ 0 false.
 Proof.
-  generalize dependent trX. generalize dependent choice.
+  generalize dependent trX. generalize dependent descriptors.
   induction tr using rev_ind; intros
   ; [inversion HtrX; subst; apply H; assumption|].
   apply finite_protocol_trace_from_app_iff in Htr. destruct Htr as [Htr Hx].
   spec IHtr Htr.
   apply equivocators_trace_project_app_iff in HtrX.
-  destruct HtrX as [trX' [xX [eqv_choice' [HxX [HtrX' HtrX]]]]].
+  destruct HtrX as [trX' [xX [eqv_descriptors' [HxX [HtrX' HtrX]]]]].
   subst trX.
   subst s. 
   simpl in HxX.
-  destruct (equivocators_transition_item_project choice x) as [(o, descriptor)|] eqn:Hpr; [|congruence].
+  destruct (equivocators_transition_item_project descriptors x) as [(o, descriptor)|] eqn:Hpr; [|congruence].
 
   inversion Hx. subst. clear Hx H3.
   destruct H4 as [[_ [_ [Hv _]]] Ht].
@@ -704,11 +755,11 @@ Proof.
   | composite_valid _ _ (?l, _) => remember l as lst
   end.
 
-  spec IHtr eqv_choice' trX' HtrX'.
+  spec IHtr eqv_descriptors' trX' HtrX'.
   apply IHtr.
 
   specialize
-    (equivocators_transition_item_project_zero_descriptor choice
+    (equivocators_transition_item_project_preserves_zero_descriptors descriptors
       {| l := l; input := iom; destination := s; output := oom |}
       o descriptor
     )
@@ -720,30 +771,32 @@ Proof.
 Qed.
 
 Lemma preloaded_equivocators_protocol_trace_from_project
-  (final_choice : equivocator_descriptors)
+  (final_descriptors : equivocator_descriptors)
   (is : composite_state equivocator_IM)
   (tr : list (composite_transition_item equivocator_IM))
   (final_state := last (map destination tr) is)
-  (Hproper : proper_equivocator_descriptors final_choice final_state)
+  (Hproper : proper_equivocator_descriptors final_descriptors final_state)
   (Htr : finite_protocol_trace_from pre_loaded_equivocators is tr)
   : exists
     (trX : list (composite_transition_item IM))
-    (initial_choice : equivocator_descriptors),
-    equivocators_trace_project final_choice tr = Some (trX, initial_choice)
-    /\ proper_equivocator_descriptors initial_choice is.
+    (initial_descriptors : equivocator_descriptors),
+    equivocators_trace_project final_descriptors tr = Some (trX, initial_descriptors)
+    /\ proper_equivocator_descriptors initial_descriptors is
+    /\ equivocators_state_project final_descriptors (last (map destination tr) is)
+     = last (map destination trX) (equivocators_state_project initial_descriptors is).
 Proof.
-  generalize dependent final_choice.
+  generalize dependent final_descriptors.
   generalize dependent is.
   induction tr using rev_ind; intros.
-  - exists []. simpl. exists final_choice. split; [reflexivity| assumption].
+  - exists []. simpl. exists final_descriptors. repeat split; assumption.
   - apply finite_protocol_trace_from_app_iff in Htr.
     destruct Htr as [Htr Hx].
     specialize (IHtr _ Htr).
-    specialize (equivocators_transition_item_project_proper_characterization final_choice x) as Hproperx.
+    specialize (equivocators_transition_item_project_proper_characterization final_descriptors x) as Hproperx.
     unfold final_state in Hproper.
     rewrite map_app in Hproper. simpl in Hproper. rewrite last_is_last in Hproper.
     spec Hproperx Hproper.
-    destruct Hproperx as [oitem [final_choice' [Hprojectx [Hitemx Hproperx]]]].
+    destruct Hproperx as [oitem [final_descriptors' [Hprojectx [Hitemx Hproperx]]]].
     specialize (Hproperx (last (map destination tr) is)).
     unfold equivocators_trace_project.
     rewrite fold_right_app.
@@ -754,34 +807,37 @@ Proof.
     rewrite Hprojectx in Heqfoldx.
     inversion Hx. subst tl s' x. clear Hx.
     destruct H3 as [[_ [_ [Hv _]]] Ht].
-    specialize (Hproperx Hv Ht). clear Hv Ht.
+    specialize (Hproperx Hv Ht).
     destruct Hproperx as [Hproper' Hx].
     specialize (IHtr _ Hproper').
-    destruct IHtr as [trX' [initial_choice [Htr_project Hproper_initial]]].
+    destruct IHtr as [trX' [initial_descriptors [Htr_project [Hproper_initial Hlst]]]].
     destruct oitem as [item|].
     + simpl in Hitemx. destruct Hitemx as [Hl [Hinput [Houtput Hdestination]]].
       specialize (Hx _ eq_refl).
       destruct Hx as [Hvx Htx].
-      exists (trX' ++ [item]), initial_choice. subst foldx.
-      rewrite equivocators_trace_project_folder_additive with (trX := trX') (eqv_descriptors := initial_choice)
+      exists (trX' ++ [item]), initial_descriptors. subst foldx.
+      rewrite equivocators_trace_project_folder_additive with (trX := trX') (eqv_descriptors := initial_descriptors)
       ; [|assumption].
-      split; [reflexivity| assumption].
-    + exists trX'. exists initial_choice. subst foldx. split; assumption.
+      repeat split; [assumption|].
+      rewrite! map_app. simpl. rewrite! last_is_last. assumption.
+    + exists trX', initial_descriptors. subst foldx. repeat split; [assumption|assumption|].
+      rewrite! map_app. simpl. rewrite! last_is_last. 
+      simpl in Hx. simpl in Hlst. congruence.
 Qed.
 
 Lemma preloaded_equivocators_protocol_trace_project_inv
-  (final_choice : equivocator_descriptors)
+  (final_descriptors : equivocator_descriptors)
   (is : composite_state equivocator_IM)
   (tr : list (composite_transition_item equivocator_IM))
   (final_state := last (map destination tr) is)
   (Htr : finite_protocol_trace pre_loaded_equivocators is tr)
   (trX : list (composite_transition_item IM))
-  (initial_choice : equivocator_descriptors)
-  (Hproject: equivocators_trace_project final_choice tr = Some (trX, initial_choice))
-  (Hproper : proper_equivocator_descriptors initial_choice is)
-  : proper_equivocator_descriptors final_choice final_state.
+  (initial_descriptors : equivocator_descriptors)
+  (Hproject: equivocators_trace_project final_descriptors tr = Some (trX, initial_descriptors))
+  (Hproper : proper_equivocator_descriptors initial_descriptors is)
+  : proper_equivocator_descriptors final_descriptors final_state.
 Proof.
-  revert Hproject. revert trX Htr final_choice.
+  revert Hproject. revert trX Htr final_descriptors.
   induction tr using rev_ind; intros; [inversion Hproject; assumption|].
   destruct Htr as [Htr Hinit].
   apply finite_protocol_trace_from_app_iff in Htr.
@@ -792,12 +848,12 @@ Proof.
   | fold_right _ ?f _ = _ => remember f as project_x
   end.
   simpl in Heqproject_x.
-  destruct project_x as [(x', x_choice)|]
+  destruct project_x as [(x', x_descriptors)|]
   ; [|rewrite equivocators_trace_project_fold_None in Hproject; congruence].
-  destruct (equivocators_transition_item_project final_choice x) as [(oitem', ditem')|]
+  destruct (equivocators_transition_item_project final_descriptors x) as [(oitem', ditem')|]
     eqn:Hproject_x
   ; [|congruence].
-  apply (equivocators_trace_project_folder_additive_iff tr x' x_choice initial_choice trX)
+  apply (equivocators_trace_project_folder_additive_iff tr x' x_descriptors initial_descriptors trX)
   in Hproject.
   destruct Hproject as [trX' [Hproject_x' HeqtrX]].
   specialize (IHtr trX' (conj Htr Hinit) _ Hproject_x').
@@ -814,7 +870,7 @@ Proof.
   unfold equivocator_vlsm_transition_item_project in Heqprojecti.
   unfold final_state in *. clear final_state.
   rewrite map_app. simpl. rewrite last_is_last.
-  destruct (final_choice (projT1 l)) as [sn| j fj] eqn:Hfinali.
+  destruct (final_descriptors (projT1 l)) as [sn| j fj] eqn:Hfinali.
   - inversion Heqprojecti. subst. clear Heqprojecti.
     inversion Hproject_x. subst; clear Hproject_x.
     inversion Heqproject_x. subst. clear Heqproject_x.
@@ -866,25 +922,29 @@ Proof.
       ).
 Qed.
 
+(**
+A corrollary of [preloaded_equivocators_protocol_trace_from_project] selecting
+only the [proper_equivocator_descriptors] property.
+*)
 Lemma preloaded_equivocators_protocol_trace_project_proper_initial
   (is : composite_state equivocator_IM)
   (tr : list (composite_transition_item equivocator_IM))
   (final_state := last (map destination tr) is)
   (Htr : finite_protocol_trace_from pre_loaded_equivocators is tr)
-  (final_choice : equivocator_descriptors)
+  (final_descriptors : equivocator_descriptors)
   (trX : list (composite_transition_item IM))
-  (initial_choice : equivocator_descriptors)
-  (Hproject: equivocators_trace_project final_choice tr = Some (trX, initial_choice))
-  (Hproper : proper_equivocator_descriptors final_choice final_state)
-  : proper_equivocator_descriptors initial_choice is.
+  (initial_descriptors : equivocator_descriptors)
+  (Hproject: equivocators_trace_project final_descriptors tr = Some (trX, initial_descriptors))
+  (Hproper : proper_equivocator_descriptors final_descriptors final_state)
+  : proper_equivocator_descriptors initial_descriptors is.
 Proof.
   destruct
     (preloaded_equivocators_protocol_trace_from_project
-      final_choice is tr Hproper Htr
+      final_descriptors is tr Hproper Htr
     )
-    as [_trX [_initial_choice [_Hproject Hiproper]]].
+    as [_trX [_initial_descriptors [_Hproject [Hiproper _]]]].
   rewrite Hproject in _Hproject.
-  inversion _Hproject. subst _trX _initial_choice.
+  inversion _Hproject. subst _trX _initial_descriptors.
   assumption.
 Qed.
 
@@ -895,10 +955,10 @@ Lemma equivocators_trace_project_output_reflecting_inv
   (m : message)
   (Hbbs : Exists (field_selector output m) tr)
   : exists
-    (final_choice initial_choice : equivocator_descriptors)
+    (final_descriptors initial_descriptors : equivocator_descriptors)
     (trX: list (composite_transition_item IM)),
-    not_equivocating_equivocator_descriptors IM final_choice (last (map destination tr) is) /\
-    equivocators_trace_project final_choice tr = Some (trX, initial_choice) /\
+    not_equivocating_equivocator_descriptors IM final_descriptors (last (map destination tr) is) /\
+    equivocators_trace_project final_descriptors tr = Some (trX, initial_descriptors) /\
     Exists (field_selector output m) trX.
 Proof.
   apply Exists_exists in Hbbs.
@@ -922,9 +982,9 @@ Proof.
   match type of Heqv_final with
   | not_equivocating_descriptor _ _ (?l i) => remember l as final
   end.
-  remember (equivocator_descriptors_update (zero_choice IM) i eqv_final) as final_choice.
-  assert (Hfinal_choice : not_equivocating_equivocator_descriptors IM final_choice final).
-  { intro eqv. subst final_choice.
+  remember (equivocator_descriptors_update (zero_descriptor IM) i eqv_final) as final_descriptors.
+  assert (Hfinal_descriptors : not_equivocating_equivocator_descriptors IM final_descriptors final).
+  { intro eqv. subst final_descriptors.
     destruct (decide (eqv = i)).
     - subst i.
       unfold equivocator_descriptors_update.  rewrite equivocator_descriptors_update_eq.
@@ -932,20 +992,20 @@ Proof.
     - unfold equivocator_descriptors_update.
       rewrite equivocator_descriptors_update_neq
       ; [|assumption].
-      apply zero_choice_proper. assumption.
+      apply zero_descriptor_proper. assumption.
   }
-  exists final_choice.
+  exists final_descriptors.
   subst final.
-  assert (Hfinal_choice_proper : proper_equivocator_descriptors final_choice (last (map Common.destination tr) is)).
+  assert (Hfinal_descriptors_proper : proper_equivocator_descriptors final_descriptors (last (map Common.destination tr) is)).
   { apply not_equivocating_equivocator_descriptors_proper. assumption. }
-  destruct (preloaded_equivocators_protocol_trace_from_project  _ _ _ Hfinal_choice_proper Htr)
-    as [trX [initial_choice [Hproject_tr _]]].
-  exists initial_choice, trX. split; [assumption|]. split; [assumption|].
+  destruct (preloaded_equivocators_protocol_trace_from_project  _ _ _ Hfinal_descriptors_proper Htr)
+    as [trX [initial_descriptors [Hproject_tr _]]].
+  exists initial_descriptors, trX. split; [assumption|]. split; [assumption|].
   specialize
-    (equivocators_trace_project_finite_trace_projection_list_commute i final_choice initial_choice
+    (equivocators_trace_project_finite_trace_projection_list_commute i final_descriptors initial_descriptors
       eqv_init tr trX trXi Hproject_tr)
     as Hcommute.
-  assert (Hfinali : final_choice i = eqv_final).
+  assert (Hfinali : final_descriptors i = eqv_final).
   { subst. apply equivocator_descriptors_update_eq. }
   rewrite Hfinali in Hcommute.
   spec Hcommute Hprojecti.
@@ -958,31 +1018,60 @@ Proof.
   simpl in *. rewrite Houtput. assumption.
 Qed.
 
+Lemma equivocators_trace_project_output_reflecting_iff
+  (is: composite_state equivocator_IM)
+  (tr: list (composite_transition_item equivocator_IM))
+  (Htr: finite_protocol_trace_from (pre_loaded_with_all_messages_vlsm (free_composite_vlsm equivocator_IM)) is tr)
+  (m : message)
+  : Exists (field_selector output m) tr
+  <-> exists
+    (final_descriptors initial_descriptors : equivocator_descriptors)
+    (trX: list (composite_transition_item IM)),
+    not_equivocating_equivocator_descriptors IM final_descriptors (last (map destination tr) is) /\
+    equivocators_trace_project final_descriptors tr = Some (trX, initial_descriptors) /\
+    Exists (field_selector output m) trX.
+Proof.
+  split; [apply equivocators_trace_project_output_reflecting_inv; assumption|].
+  intros [final_descriptors [initial_descriptors [trX [Hfinal_descriptors [Hpr_tr Hex]]]]].
+  apply Exists_exists in Hex.
+  destruct Hex as [itemX [HitemX Hm]].
+  apply in_split in HitemX.
+  destruct HitemX as [preX [sufX Heq_trX]].
+  subst.
+  apply equivocators_trace_project_app_inv_item in Hpr_tr.
+  destruct Hpr_tr as [pre [suf [item [item_descriptors [pre_descriptors [_ [Hpr_item [_ Heqtr]]]]]]]].
+  subst.
+  rewrite !Exists_app. right. left. constructor.
+  apply equivocators_transition_item_project_inv_characterization in Hpr_item.
+  destruct Hpr_item as [_ [_ [Heqoutput _]]].
+  simpl in *. congruence.
+Qed.
+
 Lemma seeded_equivocators_protocol_trace_project
-  (final_choice : equivocator_descriptors)
+  (final_descriptors : equivocator_descriptors)
   (is : vstate equivocators_no_equivocations_vlsm)
   (tr : list (composite_transition_item equivocator_IM))
   (final_state := last (map destination tr) is)
-  (Hproper : proper_equivocator_descriptors final_choice final_state)
+  (Hproper : proper_equivocator_descriptors final_descriptors final_state)
   (Htr : finite_protocol_trace SeededXE is tr)
   : exists
     (trX : list (composite_transition_item IM))
-    (initial_choice : equivocator_descriptors)
-    (isX := equivocators_state_project initial_choice is)
+    (initial_descriptors : equivocator_descriptors)
+    (isX := equivocators_state_project initial_descriptors is)
     (final_stateX := last (map destination trX) isX),
-    proper_equivocator_descriptors initial_choice is /\
-    equivocators_trace_project final_choice tr = Some (trX, initial_choice) /\
-    equivocators_state_project final_choice final_state = final_stateX /\
+    proper_equivocator_descriptors initial_descriptors is /\
+    equivocators_trace_project final_descriptors tr = Some (trX, initial_descriptors) /\
+    equivocators_state_project final_descriptors final_state = final_stateX /\
     finite_protocol_trace SeededX isX trX.
 Proof.
   remember (length tr) as len_tr.
-  generalize dependent final_choice. generalize dependent tr.
+  generalize dependent final_descriptors. generalize dependent tr.
   induction len_tr using (well_founded_induction Wf_nat.lt_wf); intros.
   subst len_tr.
   destruct_list_last tr tr' lst Htr_lst.
-  - clear H. subst. unfold final_state in *. exists [], final_choice.
+  - clear H. subst. unfold final_state in *. exists [], final_descriptors.
     split; [assumption|]. split; [reflexivity|]. split; [reflexivity|].
-    remember (equivocators_state_project final_choice is) as isx.
+    remember (equivocators_state_project final_descriptors is) as isx.
     cut (vinitial_state_prop X isx).
     { intro. split; [|assumption]. constructor.
       apply protocol_state_prop_iff. left.
@@ -997,11 +1086,11 @@ Proof.
     apply finite_protocol_trace_from_app_iff in Htr.
     destruct Htr as [Htr Hlst].
     specialize (H' tr' (conj Htr Hinit) eq_refl).
-    specialize (equivocators_transition_item_project_proper_characterization final_choice lst) as Hproperx.
+    specialize (equivocators_transition_item_project_proper_characterization final_descriptors lst) as Hproperx.
     unfold final_state in Hproper. rewrite Htr_lst in Hproper.
     rewrite map_app in Hproper. simpl in Hproper. rewrite last_is_last in Hproper.
     spec Hproperx Hproper.
-    destruct Hproperx as [oitem [final_choice' [Hprojectx [Hitemx Hproperx]]]].
+    destruct Hproperx as [oitem [final_descriptors' [Hprojectx [Hitemx Hproperx]]]].
     specialize (Hproperx (last (map destination tr') is)).
     unfold equivocators_trace_project.
     rewrite fold_right_app.
@@ -1015,13 +1104,13 @@ Proof.
     specialize (Hproperx Hv Ht). clear Hv Ht.
     destruct Hproperx as [Hproper' Hx].
     specialize (H' _ Hproper').
-    destruct H' as [trX' [initial_choice [Hproper_initial [Htr_project [Hstate_project HtrX']]]]].
+    destruct H' as [trX' [initial_descriptors [Hproper_initial [Htr_project [Hstate_project HtrX']]]]].
     destruct oitem as [item|].
     +  simpl in Hitemx. destruct Hitemx as [Hl [Hinput [Houtput Hdestination]]].
       specialize (Hx _ eq_refl).
       destruct Hx as [Hvx Htx].
-      exists (trX' ++ [item]), initial_choice. subst foldx.
-      rewrite equivocators_trace_project_folder_additive with (trX := trX') (eqv_descriptors := initial_choice)
+      exists (trX' ++ [item]), initial_descriptors. subst foldx.
+      rewrite equivocators_trace_project_folder_additive with (trX := trX') (eqv_descriptors := initial_descriptors)
       ; [|assumption].
       split; [assumption|].
       split; [reflexivity|].
@@ -1074,19 +1163,19 @@ Proof.
       }
       specialize (Hno_equiv Htr'pre eq_refl).
       destruct (equivocators_trace_project_output_reflecting_inv _ _ (proj1 Htr'pre) _ Hno_equiv)
-        as [final_choice_m [initial_choice_m [trXm [Hfinal_choice_m [Hproject_trXm Hex]]]]].
+        as [final_descriptors_m [initial_descriptors_m [trXm [Hfinal_descriptors_m [Hproject_trXm Hex]]]]].
       specialize (H (length tr')).
       spec H. { rewrite app_length. simpl. lia. }
-      assert (Hfinal_choice_m_proper : proper_equivocator_descriptors final_choice_m (last (map Common.destination tr') is))
+      assert (Hfinal_descriptors_m_proper : proper_equivocator_descriptors final_descriptors_m (last (map Common.destination tr') is))
         by (apply not_equivocating_equivocator_descriptors_proper; assumption).
-      specialize (H tr' (conj Htr Hinit) eq_refl final_choice_m Hfinal_choice_m_proper).
-      destruct H as [trXm' [initial_choice_m' [Hproper_initial_m [Hproject_trXm' [Hpr_fin_tr' HtrXm]]]]].
+      specialize (H tr' (conj Htr Hinit) eq_refl final_descriptors_m Hfinal_descriptors_m_proper).
+      destruct H as [trXm' [initial_descriptors_m' [Hproper_initial_m [Hproject_trXm' [Hpr_fin_tr' HtrXm]]]]].
       simpl in *. rewrite Hproject_trXm in Hproject_trXm'.
-      inversion Hproject_trXm'. subst trXm' initial_choice_m'. clear Hproject_trXm'.
+      inversion Hproject_trXm'. subst trXm' initial_descriptors_m'. clear Hproject_trXm'.
       repeat split; [assumption| |assumption| assumption].
       apply option_protocol_message_Some.
       apply (protocol_trace_output_is_protocol _ _ _ (proj1 HtrXm) _ Hex).
-    + exists trX'. exists initial_choice. subst foldx. split; [assumption|].
+    + exists trX'. exists initial_descriptors. subst foldx. split; [assumption|].
       split; [apply Htr_project|]. split; [|assumption].
       subst tr. clear -Hstate_project Hx.
       rewrite Hstate_project in Hx.
@@ -1095,34 +1184,34 @@ Proof.
 Qed.
 
 Lemma seeded_equivocators_protocol_trace_from_project
-  (final_choice : equivocator_descriptors)
+  (final_descriptors : equivocator_descriptors)
   (is : vstate equivocators_no_equivocations_vlsm)
   (tr : list (composite_transition_item equivocator_IM))
   (final_state := last (map destination tr) is)
-  (Hproper : proper_equivocator_descriptors final_choice final_state)
+  (Hproper : proper_equivocator_descriptors final_descriptors final_state)
   (Htr : finite_protocol_trace_from SeededXE is tr)
   : exists
     (trX : list (composite_transition_item IM))
-    (initial_choice : equivocator_descriptors)
-    (isX := equivocators_state_project initial_choice is)
+    (initial_descriptors : equivocator_descriptors)
+    (isX := equivocators_state_project initial_descriptors is)
     (final_stateX := last (map destination trX) isX),
-    proper_equivocator_descriptors initial_choice is /\
-    equivocators_trace_project final_choice tr = Some (trX, initial_choice) /\
-    equivocators_state_project final_choice final_state = final_stateX /\
+    proper_equivocator_descriptors initial_descriptors is /\
+    equivocators_trace_project final_descriptors tr = Some (trX, initial_descriptors) /\
+    equivocators_state_project final_descriptors final_state = final_stateX /\
     finite_protocol_trace_from SeededX isX trX.
 Proof.
   apply finite_protocol_trace_from_complete_left in Htr as Htr'.
   destruct Htr' as [is0 [pre [Htr' His]]].
-  apply (seeded_equivocators_protocol_trace_project final_choice) in Htr' as HtrX'
+  apply (seeded_equivocators_protocol_trace_project final_descriptors) in Htr' as HtrX'
   ; [| rewrite map_app; rewrite last_app; subst; assumption].
-  destruct HtrX' as [trX' [initial_choice' [Hinitial_choice' [Hproject' [Hstate_project HtrX']]]]].
+  destruct HtrX' as [trX' [initial_descriptors' [Hinitial_descriptors' [Hproject' [Hstate_project HtrX']]]]].
   apply equivocators_trace_project_app_iff in Hproject'.
-  destruct Hproject' as [preX [trX [initial_choice [Hproject_tr [Hproject_pre HeqtrX']]]]].
+  destruct Hproject' as [preX [trX [initial_descriptors [Hproject_tr [Hproject_pre HeqtrX']]]]].
   subst trX'.
   destruct HtrX' as [HtrX' HinitX].
   apply finite_protocol_trace_from_app_iff in HtrX'.
   destruct HtrX' as [HpreX HtrX].
-  exists trX. exists initial_choice.
+  exists trX. exists initial_descriptors.
   rewrite! map_app in Hstate_project.
   rewrite! last_app in Hstate_project.
   destruct Htr' as [Htr' Hinit].
@@ -1134,13 +1223,13 @@ Proof.
     assumption.
   }
   specialize
-    (preloaded_equivocators_protocol_trace_project_inv initial_choice _ _ HprePre _ _ Hproject_pre Hinitial_choice')
-    as Hinitial_choice.
+    (preloaded_equivocators_protocol_trace_project_inv initial_descriptors _ _ HprePre _ _ Hproject_pre Hinitial_descriptors')
+    as Hinitial_descriptors.
   destruct
-    (seeded_equivocators_protocol_trace_project _ _ _ Hinitial_choice (conj Hpre Hinit))
-    as [_preX [_initial_choice' [_ [_Hproject_pre [Hpr_last_pre _]]]]].
+    (seeded_equivocators_protocol_trace_project _ _ _ Hinitial_descriptors (conj Hpre Hinit))
+    as [_preX [_initial_descriptors' [_ [_Hproject_pre [Hpr_last_pre _]]]]].
   rewrite Hproject_pre in _Hproject_pre.
-  inversion _Hproject_pre. subst _preX _initial_choice'. clear _Hproject_pre.
+  inversion _Hproject_pre. subst _preX _initial_descriptors'. clear _Hproject_pre.
   subst is. unfold final_state in *. simpl in *. rewrite <- Hpr_last_pre in *.
   repeat (split; [assumption|]). split; [|assumption].
   match goal with
@@ -1155,25 +1244,25 @@ Qed.
 End seeded_equivocators_protocol_trace_project.
 
 Lemma equivocators_protocol_trace_from_project
-  (final_choice : equivocator_descriptors)
+  (final_descriptors : equivocator_descriptors)
   (is : vstate equivocators_no_equivocations_vlsm)
   (tr : list (composite_transition_item equivocator_IM))
   (final_state := last (map destination tr) is)
-  (Hproper : proper_equivocator_descriptors final_choice final_state)
+  (Hproper : proper_equivocator_descriptors final_descriptors final_state)
   (Htr : finite_protocol_trace_from equivocators_no_equivocations_vlsm is tr)
   : exists
     (trX : list (composite_transition_item IM))
-    (initial_choice : equivocator_descriptors)
-    (isX := equivocators_state_project initial_choice is)
+    (initial_descriptors : equivocator_descriptors)
+    (isX := equivocators_state_project initial_descriptors is)
     (final_stateX := last (map destination trX) isX),
-    proper_equivocator_descriptors initial_choice is /\
-    equivocators_trace_project final_choice tr = Some (trX, initial_choice) /\
-    equivocators_state_project final_choice final_state = final_stateX /\
+    proper_equivocator_descriptors initial_descriptors is /\
+    equivocators_trace_project final_descriptors tr = Some (trX, initial_descriptors) /\
+    equivocators_state_project final_descriptors final_state = final_stateX /\
     finite_protocol_trace_from X isX trX.
 Proof.
   specialize
     (seeded_equivocators_protocol_trace_from_project (fun m => False)
-      final_choice is tr Hproper
+      final_descriptors is tr Hproper
     ) as Hproject.
   spec Hproject.
   { apply VLSM_incl_finite_protocol_trace_from; [|assumption].
@@ -1186,8 +1275,8 @@ Proof.
     ; [intro H; apply VLSM_eq_incl_iff in H; exact (proj2 H)|].
     assumption.
   }
-  destruct Hproject as [trX [initial_choice [Hinitial_choice [Hproject_tr [Hproject_lst HtrX]]]]].
-  exists trX, initial_choice.
+  destruct Hproject as [trX [initial_descriptors [Hinitial_descriptors [Hproject_tr [Hproject_lst HtrX]]]]].
+  exists trX, initial_descriptors.
   specialize (vlsm_is_pre_loaded_with_False X) as Heq.
   apply VLSM_eq_incl_iff in Heq.
   destruct Heq as [_ Hincl].
@@ -1218,23 +1307,34 @@ Existing Instance i0.
 Existing Instance sub_i0.
 Existing Instance sub_index_eq_dec.
 
+(**
+A generalization of [equivocators_trace_project_finite_trace_projection_list_commute]
+to projections over a set of indices.
+
+We can project a trace over the composition of equivocators in two ways:
+(1) first project to a subset of equivocator components, then project that to the corresponding subset of the composition of the original components
+(2) first project to the composition of original components, then project to a subset of them
+
+The result below says that the two ways lead to the same result.
+*)
+
 Lemma equivocators_trace_project_finite_trace_sub_projection_commute
-  (final_choice initial_choice : equivocator_descriptors IM)
-  (initial_sub_choice : equivocator_descriptors (sub_IM IM selection))
+  (final_descriptors initial_descriptors : equivocator_descriptors IM)
+  (initial_sub_descriptors : equivocator_descriptors (sub_IM IM selection))
   (tr : list (composite_transition_item (equivocator_IM IM)))
   (trX : list (composite_transition_item IM))
   (tr_subX : list (composite_transition_item (sub_IM IM selection)))
-  (final_sub_choice := fun i : sub_index selection => final_choice (proj1_sig i))
-  (Hproject_tr : equivocators_trace_project IM final_choice tr = Some (trX, initial_choice))
+  (final_sub_descriptors := fun i : sub_index selection => final_descriptors (proj1_sig i))
+  (Hproject_tr : equivocators_trace_project IM final_descriptors tr = Some (trX, initial_descriptors))
   (Hproject_sub_tr :
-    equivocators_trace_project (sub_IM IM selection) final_sub_choice
+    equivocators_trace_project (sub_IM IM selection) final_sub_descriptors
       (finite_trace_sub_projection (equivocator_IM IM) selection tr)
-    = Some (tr_subX, initial_sub_choice))
-  : initial_sub_choice = (fun i => initial_choice (proj1_sig i)) /\
+    = Some (tr_subX, initial_sub_descriptors))
+  : initial_sub_descriptors = (fun i => initial_descriptors (proj1_sig i)) /\
     finite_trace_sub_projection IM selection trX = tr_subX.
 Proof.
   generalize dependent tr_subX. generalize dependent trX.
-  generalize dependent final_choice.
+  generalize dependent final_descriptors.
   induction tr using rev_ind; intros.
   - simpl in Hproject_tr. inversion Hproject_tr. subst.
     clear Hproject_tr.
@@ -1243,7 +1343,7 @@ Proof.
   - unfold equivocators_trace_project in Hproject_tr.
     rewrite fold_right_app in Hproject_tr.
     match type of Hproject_tr with
-    | fold_right _ ?i _ = _ => destruct i as [(projectx,final_choice')|] eqn:Hproject_x
+    | fold_right _ ?i _ = _ => destruct i as [(projectx,final_descriptors')|] eqn:Hproject_x
     end
     ; [|rewrite equivocators_trace_project_fold_None in Hproject_tr; inversion Hproject_tr].
     apply equivocators_trace_project_folder_additive_iff in Hproject_tr.
@@ -1251,16 +1351,16 @@ Proof.
     specialize (IHtr _ _ HtrX0).
     rewrite finite_trace_sub_projection_app in Hproject_sub_tr.
     apply equivocators_trace_project_app_iff in Hproject_sub_tr.
-    destruct Hproject_sub_tr as [tr_subX' [project_sub_x [final_sub_choice' [Hproject_sub_x [Htr_subX' Heqtr_subX]]]]].
-    assert (Hfinal_sub' : final_sub_choice' = (fun i => final_choice' (proj1_sig i)) /\ finite_trace_sub_projection IM selection projectx = project_sub_x).
+    destruct Hproject_sub_tr as [tr_subX' [project_sub_x [final_sub_descriptors' [Hproject_sub_x [Htr_subX' Heqtr_subX]]]]].
+    assert (Hfinal_sub' : final_sub_descriptors' = (fun i => final_descriptors' (proj1_sig i)) /\ finite_trace_sub_projection IM selection projectx = project_sub_x).
     { clear - Hproject_x Hproject_sub_x.
       simpl in *.
-      destruct (equivocators_transition_item_project IM final_choice x)
+      destruct (equivocators_transition_item_project IM final_descriptors x)
         as [(ox, final')|] eqn:Hpr_item_x
       ; [|congruence].
       unfold equivocators_transition_item_project in Hpr_item_x.
       unfold composite_transition_item_projection in Hpr_item_x.
-      remember (equivocator_vlsm_transition_item_project (IM (projT1 (l x))) (composite_transition_item_projection_from_eq (equivocator_IM IM) x (projT1 (l x)) eq_refl) (final_choice (projT1 (l x))))
+      remember (equivocator_vlsm_transition_item_project (IM (projT1 (l x))) (composite_transition_item_projection_from_eq (equivocator_IM IM) x (projT1 (l x)) eq_refl) (final_descriptors (projT1 (l x))))
         as pr_item_x.
       destruct pr_item_x as [(oitem', descriptor')|]; [|congruence].
       
@@ -1269,7 +1369,7 @@ Proof.
       simpl in Heqpr_item_x.
       destruct (decide (from_sub_projection (equivocator_IM IM) selection x)).
       - simpl in Hproject_sub_x.
-        unfold final_sub_choice in *.
+        unfold final_sub_descriptors in *.
         unfold equivocators_transition_item_project in Hproject_sub_x.
         match type of Hproject_sub_x with
         | context [equivocator_vlsm_transition_item_project ?X ?i ?c]
@@ -1332,7 +1432,7 @@ Proof.
               (projT1 (l x)) (l item') (l item') s f
             ).
           reflexivity.
-      - simpl in Hproject_sub_x. unfold final_sub_choice in *.
+      - simpl in Hproject_sub_x. unfold final_sub_descriptors in *.
         inversion Hproject_sub_x. subst. clear Hproject_sub_x.
         split.
         + apply functional_extensionality_dep. intros i.
@@ -1354,7 +1454,7 @@ Proof.
           reflexivity.
     }
     destruct Hfinal_sub' as [Hfinal_sub' Hpr_sub_x].
-    subst final_sub_choice'.
+    subst final_sub_descriptors'.
     specialize (IHtr _ Htr_subX').
     destruct IHtr as [Heqv_initial Hpr_trXi'].
     split; [assumption|].
